books/centaur/aig/aig-equivs.lisp
@@ -1,55 +1,118 @@
+; Centaur AIG Library
+; Copyright (C) 2008-2011 Centaur Technology
+;
+; Contact:
+;   Centaur Technology Formal Verification Group
+;   7600-C N. Capital of Texas Highway, Suite 300, Austin, TX 78731, USA.
+;   http://www.centtech.com/
+;
+; This program is free software; you can redistribute it and/or modify it under
+; the terms of the GNU General Public License as published by the Free Software
+; Foundation; either version 2 of the License, or (at your option) any later
+; version.  This program is distributed in the hope that it will be useful but
+; WITHOUT ANY WARRANTY; without even the implied warranty of MERCHANTABILITY or
+; FITNESS FOR A PARTICULAR PURPOSE.  See the GNU General Public License for
+; more details.  You should have received a copy of the GNU General Public
+; License along with this program; if not, write to the Free Software
+; Foundation, Inc., 51 Franklin Street, Suite 500, Boston, MA 02110-1335, USA.
+;
+; Original author: Sol Swords <sswords@centtech.com>
 
 (in-package "ACL2")
 
 (include-book "base")
 (include-book "centaur/misc/witness-cp" :dir :system)
 (include-book "centaur/misc/universal-equiv" :dir :system)
+(include-book "centaur/misc/fast-alists" :dir :system)
+(set-verify-guards-eagerness 0)
 
-(def-universal-equiv aig-equiv
-  :qvars env
-  :equiv-terms ((equal (aig-eval x env)))
-  :defquant t
-  :witness-dcls ((declare (xargs :guard t
-                                 :verify-guards nil))))
 
-(verify-guards aig-equiv)
+(defsection aig-equiv
+  :parents (aig)
+  :short "We say the AIGs <tt>X</tt> and <tt>Y</tt> are equivalent when they
+always evaluate to the same value, per @(see aig-eval)."
+  :long "@(def aig-equiv)"
 
-(def-universal-equiv aig-alist-equiv
-  :qvars k
-  :equiv-terms ((iff (hons-assoc-equal k x))
-                (aig-equiv (cdr (hons-assoc-equal k x))))
-  :defquant t
-  :witness-dcls ((declare (xargs :guard t
-                                 :verify-guards nil))))
+  (def-universal-equiv aig-equiv
+    :qvars env
+    :equiv-terms ((equal (aig-eval x env)))
+    :defquant t
+    :witness-dcls ((declare (xargs :guard t))))
 
-(verify-guards aig-alist-equiv)
+  (verify-guards aig-equiv))
 
-(def-universal-equiv faig-equiv
-  :qvars env
-  :equiv-terms ((equal (faig-eval x env)))
-  :defquant t
-  :witness-dcls ((declare (xargs :guard t
-                                 :verify-guards nil))))
 
-(verify-guards faig-equiv)
 
-(def-universal-equiv faig-alist-equiv
-  :qvars k
-  :equiv-terms ((iff (hons-assoc-equal k x))
-                (faig-equiv (cdr (hons-assoc-equal k x))))
-  :defquant t
-  :witness-dcls ((declare (xargs :guard t
-                                 :verify-guards nil))))
+(defsection aig-alist-equiv
+  :parents (aig)
+  :short "We say the AIG Alists <tt>X</tt> and <tt>Y</tt> are equivalent when
+they bind the same keys to equivalent AIGs, in the sense of @(see aig-equiv)."
+  :long "@(def aig-alist-equiv)"
 
-(verify-guards faig-alist-equiv)
+  (def-universal-equiv aig-alist-equiv
+    :qvars k
+    :equiv-terms ((iff (hons-assoc-equal k x))
+                  (aig-equiv (cdr (hons-assoc-equal k x))))
+    :defquant t
+    :witness-dcls ((declare (xargs :guard t))))
 
-(def-universal-equiv aig-env-equiv
-  :qvars key
-  :equiv-terms ((iff (aig-env-lookup key x)))
-  :defquant t
-  :witness-dcls ((declare (xargs :guard t
-                                 :verify-guards nil))))
+  (verify-guards aig-alist-equiv)
 
-(verify-guards aig-env-equiv)
+  (defrefinement alist-equiv aig-alist-equiv
+    :hints ((witness))))
+
+
+
+
+(defsection aig-env-equiv
+  :parents (aig)
+  :short "We say the environments <tt>X</tt> and <tt>Y</tt> are equivalent when
+they give equivalent values to variables looked up with @(see aig-env-lookup)."
+  :long "@(def aig-env-equiv)"
+
+  (def-universal-equiv aig-env-equiv
+    :qvars key
+    :equiv-terms ((iff (aig-env-lookup key x)))
+    :defquant t
+    :witness-dcls ((declare (xargs :guard t))))
+
+  (verify-guards aig-env-equiv)
+
+  (defrefinement alist-equiv aig-env-equiv
+    :hints ((witness))))
+
+
+
+
+(defsection faig-equiv
+  :parents (faig)
+  :short "We say the FAIGs <tt>X</tt> and <tt>Y</tt> are equivalent when they
+always evaluate to the same value, per @(see faig-eval)."
+
+  (def-universal-equiv faig-equiv
+    :qvars env
+    :equiv-terms ((equal (faig-eval x env)))
+    :defquant t
+    :witness-dcls ((declare (xargs :guard t))))
+
+  (verify-guards faig-equiv))
+
+
+(defsection faig-alist-equiv
+  :parents (faig)
+  :short "We say the FAIG Alists <tt>X</tt> and <tt>Y</tt> are equivalent when
+they bind the same keys to equivalent FAIGs, in the sense of @(see faig-equiv)."
+
+  (def-universal-equiv faig-alist-equiv
+    :qvars k
+    :equiv-terms ((iff (hons-assoc-equal k x))
+                  (faig-equiv (cdr (hons-assoc-equal k x))))
+    :defquant t
+    :witness-dcls ((declare (xargs :guard t))))
+
+  (verify-guards faig-alist-equiv)
+
+  (defrefinement alist-equiv faig-alist-equiv
+    :hints ((witness))))
 
 
