books/centaur/aig/base.lisp
@@ -1,194 +1,1264 @@
+; Centaur AIG Library
+; Copyright (C) 2008-2011 Centaur Technology
+;
+; Contact:
+;   Centaur Technology Formal Verification Group
+;   7600-C N. Capital of Texas Highway, Suite 300, Austin, TX 78731, USA.
+;   http://www.centtech.com/
+;
+; This program is free software; you can redistribute it and/or modify it under
+; the terms of the GNU General Public License as published by the Free Software
+; Foundation; either version 2 of the License, or (at your option) any later
+; version.  This program is distributed in the hope that it will be useful but
+; WITHOUT ANY WARRANTY; without even the implied warranty of MERCHANTABILITY or
+; FITNESS FOR A PARTICULAR PURPOSE.  See the GNU General Public License for
+; more details.  You should have received a copy of the GNU General Public
+; License along with this program; if not, write to the Free Software
+; Foundation, Inc., 51 Franklin Street, Suite 500, Boston, MA 02110-1335, USA.
+;
+; Original author: Sol Swords <sswords@centtech.com>
+;
+; July 2011, Jared added lots of documentation.
 
 (in-package "ACL2")
+(include-book "cutil/defsection" :dir :system)
 
-(defdoc aig
-  ":doc-section aig
-AIG library for ACL2.~/
+; aig/base.lisp
+;   - Semantics of AIGs (aig-eval) and FAIGs (faig-eval)
+;   - Primitive AIG constructors (aig-not, aig-and, ...)
+;   - Substitution operations: aig-restrict, aig-compose, aig-partial-eval
+;   - FAIG versions of the substitution operations
 
-An AIG (And/Inverter Graph) is a Boolean function representation that consists
-of AND nodes and inversions.  We represent AIGs in ACL2 as cons trees, with the
-following meanings.
 
-T represents the constant-true function
+; BOZO consider using defprojection throughout?
 
-NIL represents the constant-false function
+(defxdoc aig
+  :short "Centaur AIG Library"
 
-Non-Boolean atoms represent Boolean variables (inputs)
+  :long "<p><b>AIGs</b> (And/Inverter Graphs) are a representation of Boolean
+functions, using only <i>and</i> and <i>not</i> operations.</p>
 
-A cons whose cdr is NIL represents the negation of its car, and
+<p><b><see topic='@(url faig)'>FAIGs</see></b> (Four-valued AIGs) are a related
+concept, where two AIGs are pasted together to represent a function in
+four-valued logic.</p>
 
-A cons whose cdr is non-NIL represents the AND of its car and cdr.
 
-Basic functions for operating on AIGs include aig-not, aig-and, aig-or,
-aig-ite, etc.  An AIG may be evaluated under an assignment to its variables
-(represented as a fast alist binding those variables to Booleans) using
-aig-eval.
-~/~/")
+<h3>Motivation for AIGs</h3>
 
-;; AIGs.
-;; an AIG is any of:
+<p>There are many ways to represent Boolean functions.  One alternative is
+to use BDDs, e.g., we provide a @(see ubdds) library.  In comparison with
+BDDs, AIGs are:</p>
 
-;; TRUE, represented as t
-;; FALSE, represented as nil
-;; a VARIABLE, represented as any atom other than t or nil.
-;; an INV of one AIG, represented as a cons with nil cdr
-;; an AND of two AIGs, represented as a cons of two AIGs.
+<ul>
 
-;; (Thus every ACL2 object is an AIG.)
+<li>cheaper to construct, e.g., if we want to <i>or</i> together the functions
+<tt>f</tt> and <tt>g</tt>, it only takes a few conses with AIGs, whereas with
+BDDs we need to walk through <tt>f</tt> and <tt>g</tt> to construct a new
+structure (which might be quite large); but</li>
 
-;; Note that these next two functions are provably equal to T.
-(defn aigp (x)
-  (or
-   (atom x)
-   (and (consp x) (null (cdr x)))
-   (and (aigp (car x)) (aigp (cdr x))))
-  )
+<li>more expensive to compare, e.g., with BDDs we can determine if <tt>f</tt>
+and <tt>g</tt> are equal via pointer equality, whereas with AIGs this is a
+satisfiablity problem.</li>
 
-(defn aig-listp (x)
-  (if (consp x)
-      (and
-       (aigp (car x))
-       (aig-listp (cdr x)))
-    t))   
+</ul>
 
-(defmacro aig-cases (x &key true false var inv and)
-  `(let ((aig-cases-var ,x))
-     (cond
-      ((eq aig-cases-var t) ,true)
-      ((eq aig-cases-var nil) ,false)
-      ((atom aig-cases-var) ,var)
-      ((eq (cdr aig-cases-var) nil) ,inv)
-      (t ,and))))
+<p>This tradeoff is often worth it because you can simplify and reduce AIGs
+after they have been constructed, but before comparing them.  For instance, our
+@(see bddify) algorithm converts an AIG into a BDD, and since it can often
+\"prune\" branches of the AIG that turn out to be irrelevant, it can be much
+more efficient than directly constructing BDDs.  A more sophisticated tool is
+@(see abc), which provides various kinds of rewriting and reductions on AIGs.
+These reductions can be used before calling a SAT solver or <tt>bddify</tt> to
+make the input AIGs much smaller and easier to process.</p>
 
-(defn aig-not (x)
-  (aig-cases
-   x
-   :true nil
-   :false t
-   :var (hons x nil)
-   :inv (car x)
-   :and (hons x nil)))
+<p>Another alternative would be to use a richer language such as Lisp-style
+s-expressions, where operations other than <i>and</i> and <i>not</i> could be
+used directly.  On the surface, this approach would appear to be more compact,
+e.g., we can represent <tt>(or a b)</tt> as a single operation instead of as
+something like <tt>(not (and (not a) (not b)))</tt>.</p>
 
-(defn aig-and (x y)
-  (cond
-   ((or (eq x nil) (eq y nil)) nil)
-   ((eq x t) y)
-   ((eq y t) x)
-   ((hons-equal x y) x)
-   ((and (consp y) (eq (cdr y) nil)
-         (hons-equal (car y) x))
+<p>But another critical part of memory efficiency is structure sharing.  That
+is, suppose that we already need <tt>(not a)</tt> and <tt>(not b)</tt>
+elsewhere in the function.  With s-expressions, these terms would have nothing
+in common with <tt>(or a b)</tt>, but with AIGs we can reuse the existing parts
+of <tt>(not (and (not a) (not b)))</tt>.</p>
+
+
+<h3>Representation of AIGs</h3>
+
+<p>We always construct AIGs with @(see hons) so that existing pieces of AIGs
+will be automatically reused.  We represent AIGs as arbitrary cons trees, which
+we interpret as follows:</p>
+
+<ul>
+
+<li><tt>T</tt> represents the constant-true function.</li>
+
+<li><tt>NIL</tt> represents the constant-false function.</li>
+
+<li>Any other atom represents a Boolean variable (i.e., an input to the
+function.)</li>
+
+<li>A cons of the form <tt>(A . NIL)</tt> represents the negation of
+<tt>A</tt>.</li>
+
+<li>Any other cons, <tt>(A . B)</tt>, represents the conjunction of <tt>A</tt>
+and <tt>B</tt>.</li>
+
+</ul>
+
+<p>This meaning of cons trees is given by the evaluation function @(see
+aig-eval), which returns the (Boolean) value of an AIG under some particular
+assignment to its variables.  Note that every ACL2 object is a well-formed AIG
+under this definition.</p>
+
+
+<h3>Library Functions</h3>
+
+<p>We provide some basic, low-level @(see aig-constructors) for building
+AIGs (<i>and</i>, <i>or</i>, etc.).  We prove these operations correct with
+respect to @(see aig-eval).</p>
+
+<p>There are also higher-level operations such as @(see aig-restrict) and @(see
+aig-compose) allow you to substitute into AIGs.</p>
+
+<p>It is often important to know which variables occur in an AIG.  One way to
+do this is with @(see aig-vars).</p>
+
+<p>The @(see bddify) algorithm provides a way to construct a BDD from an AIG.
+This is also used as the basis for an efficient @(see GL) symbolic counterpart
+of @(see aig-eval).</p>
+
+<p>BOZO other things that we haven't released yet.</p>")
+
+
+
+; -----------------------------------------------------------------------------
+;
+;                            EVALUATING AIGS
+;
+; -----------------------------------------------------------------------------
+
+(defsection aig-env-lookup-missing-output
+  :parents (aig-eval)
+  :short "Stub for warnings about missing variables in AIG evaluation."
+
+  :long "<p>This stub is called when @(see aig-eval) encounters a variable in
+the AIG that has no binding in the environment.  It is generally configured
+with @(see aig-env-lookup-missing-action).</p>"
+
+  (defstub aig-env-lookup-missing-output (name) nil))
+
+
+(defsection aig-env-lookup-missing-action
+  :parents (aig-eval)
+  :short "Configure warnings about missing variables in AIG evaluation."
+
+  :long "<p>Ordinarily @(see aig-eval) treats any variables that are not bound
+in the environment as having value <tt>t</tt>.  But a missing bindings could be
+the result of a bug in your program, so by default <tt>aig-eval</tt> is set up
+to print a warning if this happens.</p>
+
+<p>@(call aig-env-lookup-missing-action) allows you to control whether these
+warnings are printed, and also whether @(see break$) should be called.  The
+valid <tt>action</tt>s are:</p>
+
+<ul>
+ <li><tt>nil</tt>, silently bind the variable to <tt>t</tt>,</li>
+ <li><tt>:warn</tt> (the default), print a warning but do not <tt>break$</tt>, and</li>
+ <li><tt>:break</tt>, to print the warning and then call <tt>break$</tt>.</li>
+</ul>"
+
+  (defconst *aig-env-lookup-warn-missing-binding*
+    ;; Even with the stub and defattach, it is useful to have this "constant"
+    ;; so that, in raw lisp, we can use a let-binding to disable missing output
+    ;; warnings temporarily, e.g., so that if a SAT solver produces an
+    ;; incomplete counterexample, we don't print warnings when we check it.
+    ;; Doing this with defattach directly would be hard/impossible due to
+    ;; attachment being an event.
+    t)
+
+  (defun aig-env-lookup-missing-quiet (name)
+    (declare (xargs :guard t) (ignore name))
     nil)
-   ((and (consp x) (eq (cdr x) nil)
-         (hons-equal (car x) y))
-    nil)
-   (t (hons x y))))
+
+  (defun aig-env-lookup-missing-complain (name)
+    (declare (xargs :guard t))
+    (and *aig-env-lookup-warn-missing-binding*
+         (cw "WARNING: Missing variable binding ~x0 in AIG-ENV-LOOKUP; ~
+              assigning T~%"
+             name)))
+
+  (local (in-theory (disable (break$))))
+
+  (defun aig-env-lookup-missing-break (name)
+    (declare (xargs :guard t))
+    (and *aig-env-lookup-warn-missing-binding*
+         (prog2$ (cw "WARNING: Missing variable binding ~x0 in ~x1; assigning ~
+                      T. To avoid this break, run ~x2, where action is NIL or ~
+                      :WARN.~%"
+                     name
+                     'aig-env-lookup
+                     '(aig-env-lookup-missing-action action))
+                 (break$))))
+
+  (defmacro aig-env-lookup-missing-action (val)
+    (case val
+      ((nil) '(defattach aig-env-lookup-missing-output
+                aig-env-lookup-missing-quiet))
+      (:warn '(defattach aig-env-lookup-missing-output
+                aig-env-lookup-missing-complain))
+      (:break '(defattach aig-env-lookup-missing-output
+                 aig-env-lookup-missing-break))
+      (t (er hard 'aig-env-lookup-missing-action
+             "Expected argument NIL, :WARN, or :BREAK.~%"))))
+
+  (aig-env-lookup-missing-action :warn))
+
+
+(defsection aig-cases
+  :parents (aig)
+  :short "Control-flow macro to split into cases on what kind of AIG you have
+encountered."
+
+  (defmacro aig-cases (x &key true false var inv and)
+    `(let ((aig-cases-var ,x))
+       (cond
+        ((eq aig-cases-var t) ,true)
+        ((eq aig-cases-var nil) ,false)
+        ((atom aig-cases-var) ,var)
+        ((eq (cdr aig-cases-var) nil) ,inv)
+        (t ,and)))))
 
 
 
-(defstub aig-env-lookup-missing-output (name) nil)
+(defsection aig-eval
+  :parents (aig)
+  :short "@(call aig-eval) evaluates <tt>x</tt>, an @(see aig), under the
+environment <tt>env</tt>, producing a Boolean result."
 
-(defun aig-env-lookup-missing-quiet (name)
-  (declare (xargs :guard t) (ignore name))
-  nil)
+  :long "<p>The <tt>env</tt> should be a fast alist (see @(see fast-alists))
+that binds variables in the AIG to values.  Typically it should bind every
+variable in the AIG to a Boolean value.</p>
+
+<p>This function is @(see memoize)d.  You should typically free its memo table
+after you are done with whatever <tt>env</tt> you are using, to avoid excessive
+memory usage.  (We don't use <tt>:forget t</tt> because you often want to
+evaluate several related AIGs.)</p>
+
+<p>Unbound variables are given the default value <tt>t</tt> instead of
+<tt>nil</tt> because this makes theorems about @(see faig) evaluation work out
+more nicely (it makes unbound FAIG variables evaluate to <tt>X</tt>).</p>
+
+<p>This function essentially defines the semantics of AIGs.</p>"
+
+  ;; [Jared] BOZO it might be good to add a check that the variables are indeed
+  ;; bound to Booleans.
+
+  (defun aig-env-lookup (x env)
+    (declare (xargs :guard t))
+    (let ((look (hons-get x env)))
+      (if look
+          ;; [Jared] I was once tempted to change this to produce an always
+          ;; Boolean result, since it would seem nicer to do that here than in
+          ;; aig-eval.  But this function is also used in AIG-COMPOSE, and it
+          ;; is not valid to Boolean-fix it there.
+          (cdr look)
+        (mbe :logic t
+             :exec
+             (if *aig-env-lookup-warn-missing-binding*
+                 (prog2$ (aig-env-lookup-missing-output x)
+                         t)
+               t)))))
+
+  (defun aig-eval (x env)
+    (declare (xargs :guard t))
+    (aig-cases x
+               :true t
+               :false nil
+               :var (and (aig-env-lookup x env) t)
+               :inv (not (aig-eval (car x) env))
+               :and (and (aig-eval (car x) env)
+                         (aig-eval (cdr x) env))))
+
+  ;; [Jared] note, changed memoization condition from just (consp x) to exclude
+  ;; not nodes; this matches aig-vars and I think is probably what we want.
+  (memoize 'aig-eval :condition '(and (consp x) (cdr x))))
 
 
-(defconst *aig-env-lookup-warn-missing-binding* t)
+(defsection aig-eval-list
+  :parents (aig-eval)
+  :short "@(call aig-eval-list) evaluates a list of AIGs."
 
-(defun aig-env-lookup-missing-complain (name)
+  ;; BOZO formal is named benv right now, eventually rename to env but we need
+  ;; to patch up GL so it doesn't care about formals named env.
+  (defun aig-eval-list (x benv)
+    (declare (xargs :guard t))
+    (if (atom x)
+        nil
+      (cons (aig-eval (car x) benv)
+            (aig-eval-list (cdr x) benv)))))
+
+
+(defsection aig-eval-alist
+  :parents (aig-eval)
+  :short "@(call aig-eval-alist) evaluates an AIG Alist (an alist binding keys
+to AIGs)."
+
+  :long "<p>The alist <tt>x</tt> does not need to be fast, and we produce an
+ordinary (slow) alist as a result.</p>"
+
+  (defun aig-eval-alist (x env)
+    (declare (xargs :guard t))
+    (cond ((atom x)
+           nil)
+          ((atom (car x))
+           ;; Bad-alist convention
+           (aig-eval-alist (cdr x) env))
+          (t
+           (cons (cons (caar x) (aig-eval (cdar x) env))
+                 (aig-eval-alist (cdr x) env))))))
+
+
+
+(defsection aig-eval-alists
+  :parents (aig-eval)
+  :short "Evaluate a list of AIG Alists."
+
+  (defun aig-eval-alists (x env)
+    (declare (xargs :guard t))
+    (if (atom x)
+        nil
+      (cons (aig-eval-alist (car x) env)
+            (aig-eval-alists (cdr x) env)))))
+
+
+
+
+; -----------------------------------------------------------------------------
+;
+;                        COLLECTING AIG VARIABLES
+;
+; -----------------------------------------------------------------------------
+
+(defsection hons-alphorder-merge
+  :parents (aig-vars)
+  :short "Merge two already-@(see alphorder)ed lists of atoms."
+
+  :long "<p>This is a completely standard ordered-union operation.  Since we
+often use symbols as variables, and since alphorder puts the symbolp case far
+down after many other type checks, we use our own <tt>fast-alphorder</tt> that
+optimizes for symbols.</p>"
+
+;; BOZO maybe release the proof from nat-var-sexprs.lisp that this is just
+;; sets::union for sets of atoms.
+
+  (defabbrev fast-alphorder (x y)
+    (mbe :logic (alphorder x y)
+         :exec
+         (if (and (symbolp x)
+                  (symbolp y))
+             (or (eq x y)
+                 (not (symbol-< y x)))
+           (alphorder x y))))
+
+  (defun hons-alphorder-merge (a b)
+    (declare (xargs :guard (and (atom-listp a)
+                                (atom-listp b))
+                    :guard-hints(("Goal" :in-theory (enable alphorder symbol-<)))
+                    :measure (+ (len a) (len b))))
+    (cond ((atom a) b)
+          ((atom b) a)
+          ((equal (car a) (car b))
+           (hons-alphorder-merge (cdr a) b))
+          ((fast-alphorder (car b) (car a))
+           (hons (car b) (hons-alphorder-merge a (cdr b))))
+          (t (hons (car a) (hons-alphorder-merge (cdr a) b)))))
+
+  (memoize 'hons-alphorder-merge
+           :condition '(or (consp a) (consp b))
+           :inline nil)
+
+  (defthm atom-listp-hons-alphorder-merge
+    (implies (and (atom-listp a)
+                  (atom-listp b))
+             (atom-listp (hons-alphorder-merge a b)))
+    :hints(("Goal" :in-theory (enable hons-alphorder-merge
+                                      atom-listp))))
+
+  (defthm member-equal-hons-alphorder-merge
+    (iff (member-equal k (hons-alphorder-merge a b))
+         (or (member-equal k a)
+             (member-equal k b)))))
+
+
+(defsection aig-vars
+  :parents (aig)
+  :short "@(call aig-vars) returns the list of variables used in the AIG
+<tt>X</tt>."
+
+;; BOZO the :long here refers to the unreleased sexpr library, but I don't want
+;; to redo all that documentation for AIGs.
+
+  :long "<p>This is one scheme for collecting variables from an AIG.  We
+memoize the whole computation and return ordered lists so that merging is
+linear.  This can be very expensive.  See @(see sexpr-vars) for an analagous
+discussion.</p>"
+
+  (defun aig-vars (x)
+    (declare (xargs :guard t
+                    :verify-guards nil))
+    (aig-cases x
+               :true  nil
+               :false nil
+               :var   (hons x nil)
+               :inv   (aig-vars (car x))
+               :and   (hons-alphorder-merge (aig-vars (car x))
+                                            (aig-vars (cdr x)))))
+
+  (defthm atom-listp-aig-vars
+    (atom-listp (aig-vars x)))
+
+  (verify-guards aig-vars)
+
+  (memoize 'aig-vars :condition '(and (consp x) (cdr x))))
+
+
+
+
+; -----------------------------------------------------------------------------
+;
+;                              AIG CONSTRUCTION
+;
+; -----------------------------------------------------------------------------
+
+(defxdoc aig-constructors
+  :parents (aig)
+  :short "Low-level functions for constructing AIGs.")
+
+
+
+(defsection aig-not
+  :parents (aig-constructors)
+  :short "@(call aig-not) constructs an AIG representing <tt>(not x)</tt>."
+
+  :long "<p>This could be implemented as <tt>(hons x nil)</tt>, but we at least
+take care to fold constants and avoid creating double negatives.</p>"
+
+  (defund aig-not (x)
+    (declare (xargs :guard t))
+    (cond ((eq x nil) t)
+          ((eq x t) nil)
+          ((and (consp x) (eq (cdr x) nil))
+           (car x))
+          (t
+           (hons x nil))))
+
+  (local (in-theory (enable aig-not)))
+
+  (defthm aig-eval-not
+    (equal (aig-eval (aig-not x) env)
+           (not (aig-eval x env)))))
+
+
+
+(defsection aig-and
+  :parents (aig-constructors)
+  :short "@(call aig-and) constructs an AIG representing <tt>(and x y)</tt>."
+
+  :long "<p>This could have been implemented as <tt>(hons x y)</tt>, but we
+take care to fold constants and reduce <tt>x &amp; x</tt> and <tt>x &amp;
+~x</tt>.</p>"
+
+  (defund aig-and (x y)
+    (declare (xargs :guard t))
+    (cond
+     ((or (eq x nil) (eq y nil)) nil)
+     ((eq x t) y)
+     ((eq y t) x)
+     ((hons-equal x y) x)
+     ((and (consp y) (eq (cdr y) nil)
+           (hons-equal (car y) x))
+      nil)
+     ((and (consp x) (eq (cdr x) nil)
+           (hons-equal (car x) y))
+      nil)
+     (t (hons x y))))
+
+  (local (in-theory (enable aig-and)))
+
+  (defthm aig-eval-and
+    (equal (aig-eval (aig-and x y) env)
+           (and (aig-eval x env)
+                (aig-eval y env))))
+
+  (defthm aig-and-constants
+    (and (equal (aig-and nil x) nil)
+         (equal (aig-and x nil) nil)
+         (equal (aig-and x t) x)
+         (equal (aig-and t x) x))))
+
+
+
+(defsection aig-or
+  :parents (aig-constructors)
+  :short "@(call aig-or) constructs an AIG representing <tt>(or x y)</tt>."
+
+  (defund aig-or (x y)
+    (declare (xargs :guard t))
+    (aig-not (aig-and (aig-not x) (aig-not y))))
+
+  (local (in-theory (enable aig-or)))
+
+  (defthm aig-eval-or
+    (equal (aig-eval (aig-or x y) env)
+           (or (aig-eval x env)
+               (aig-eval y env)))))
+
+
+
+(defsection aig-xor
+  :parents (aig-constructors)
+  :short "@(call aig-xor) constructs an AIG representing <tt>(xor x y)</tt>."
+
+  (defund aig-xor (x y)
+    (declare (xargs :guard t))
+    (aig-or (aig-and x (aig-not y))
+            (aig-and (aig-not x) y)))
+
+  (local (in-theory (enable aig-xor)))
+
+  (defthm aig-eval-xor
+    (equal (aig-eval (aig-xor x y) env)
+           (xor (aig-eval x env)
+                (aig-eval y env)))))
+
+
+
+(defsection aig-iff
+  :parents (aig-constructors)
+  :short "@(call aig-iff) constructs an AIG representing <tt>(iff x y)</tt>."
+
+  (defund aig-iff (x y)
+    (declare (xargs :guard t))
+    (aig-or (aig-and x y)
+            (aig-and (aig-not x) (aig-not y))))
+
+  (local (in-theory (enable aig-iff)))
+
+  (defthm aig-eval-iff
+    (equal (aig-eval (aig-iff x y) env)
+           (iff (aig-eval x env)
+                (aig-eval y env)))))
+
+
+
+(defsection aig-implies
+  :parents (aig-constructors)
+  :short "@(call aig-implies) constructs an AIG representing <tt>(implies x y)</tt>."
+
+  (defund aig-implies (x y)
+    (declare (xargs :guard t))
+    (aig-not (aig-and x (aig-not y))))
+
+  (local (in-theory (enable aig-implies)))
+
+  (defthm aig-eval-implies
+    (equal (aig-eval (aig-implies x y) env)
+           (implies (aig-eval x env)
+                    (aig-eval y env)))))
+
+
+
+(defsection aig-ite
+  :parents (aig-constructors)
+  :short "@(call aig-ite) constructs an AIG representing <tt>(if a b c)</tt>."
+
+  (defund aig-ite (a b c)
+    (declare (xargs :guard t))
+    (cond ((hons-equal b c)
+           b)
+          ((eq b t)
+           (aig-or a c))
+          (t
+           (aig-or (aig-and a b)
+                   (aig-and (aig-not a) c)))))
+
+  (local (in-theory (enable aig-ite)))
+
+  (defthm aig-eval-ite
+    (iff (aig-eval (aig-ite a b c) env)
+         (if (aig-eval a env)
+             (aig-eval b env)
+           (aig-eval c env)))))
+
+
+(defsection aig-not-list
+  :parents (aig-constructors)
+  :short "@(call aig-not-list) negates every AIG in the list <tt>x</tt>."
+
+  (defun aig-not-list (x)
+    (declare (xargs :guard t))
+    (if (atom x)
+        nil
+      (cons (aig-not (car X))
+            (aig-not-list (cdr x))))))
+
+
+(defsection aig-and-list
+  :parents (aig-constructors)
+  :short "@(call aig-and-list) ands together all of the AIGs in the list
+<tt>x</tt>."
+
+  (defun aig-and-list (x)
+    (declare (xargs :guard t))
+    (if (atom x)
+        t
+      (aig-and (car x)
+               (aig-and-list (cdr x))))))
+
+
+(defsection aig-or-list
+  :parents (aig-constructors)
+  :short "@(call aig-or-list) ors together all of the AIGs in the list
+<tt>x</tt>."
+
+  (defun aig-or-list (x)
+    (declare (xargs :guard t))
+    (if (atom x)
+        nil
+      (aig-or (car x) (aig-or-list (cdr x))))))
+
+
+(defsection aig-and-lists
+  :parents (aig-constructors)
+  :short "@(call aig-and-lists) pairwise <i>and</i>s together the AIGs from the
+lists <tt>x</tt> and <tt>y</tt>."
+
+  (defun aig-and-lists (x y)
+    (if (or (atom x) (atom y))
+        nil
+      (cons (aig-and (car x) (car y))
+            (aig-and-lists (cdr x) (cdr y))))))
+
+
+(defsection aig-or-lists
+  :parents (aig-constructors)
+  :short "@(call aig-or-lists) pairwise <i>or</i>s together the AIGs from the
+lists <tt>x</tt> and <tt>y</tt>."
+
+  (defun aig-or-lists (x y)
+    (declare (xargs :guard t))
+    (if (or (atom x) (atom y))
+        nil
+      (cons (aig-or (car x) (car y))
+            (aig-or-lists (cdr x) (cdr y))))))
+
+
+(defsection aig-iff-lists
+  :parents (aig-constructors)
+  :short "@(call aig-iff-lists) pairwise <i>iff</i>s together the AIGs from the
+lists <tt>x</tt> and <tt>y</tt>."
+
+  (defun aig-iff-lists (x y)
+    (declare (xargs :guard t))
+    (if (or (atom x) (atom y))
+        nil
+      (cons (aig-iff (car x) (car y))
+            (aig-iff-lists (cdr x) (cdr y))))))
+
+
+(defsection aig-xor-lists
+  :parents (aig-constructors)
+  :short "@(call aig-xor-lists) pairwise <i>xor</i>s together the AIGs from the
+lists <tt>x</tt> and <tt>y</tt>."
+
+  (defun aig-xor-lists (x y)
+    (declare (xargs :guard t))
+    (if (or (atom x) (atom y))
+        nil
+      (cons (aig-xor (car x) (car y))
+            (aig-xor-lists (cdr x) (cdr y))))))
+
+
+(defsection aig-implies-lists
+  :parents (aig-constructors)
+  :short "@(call aig-implies-lists) pairwise <i>implies</i> together the AIGs from the
+lists <tt>x</tt> and <tt>y</tt>."
+
+  (defun aig-implies-lists (x y)
+    (declare (xargs :guard t))
+    (if (or (atom x) (atom y))
+        nil
+      (cons (aig-implies (car x) (car y))
+            (aig-implies-lists (cdr x) (cdr y))))))
+
+
+
+
+; -----------------------------------------------------------------------------
+;
+;                         SUBSTITUTION INTO AIGS
+;
+; -----------------------------------------------------------------------------
+
+(defsection aig-restrict
+  :parents (aig)
+  :short "@(call aig-restrict) performs variable substitution throughout the
+AIG <tt>x</tt>, replacing any variables bound in <tt>sigma</tt> with their
+corresponding values."
+
+  :long "<p><tt>sigma</tt> should be a fast alist; its name is intended to
+evoke the notion of substitution lists in logic.  Any variables that are not
+mentioned in <tt>sigma</tt> are left unchanged.</p>
+
+<p>This function is @(see memoize)d.  You should typically free its memo table
+after you are done with whatever <tt>sigma</tt> you are using, to avoid
+excessive memory usage.  (We don't use <tt>:forget t</tt> because you often
+want to restrict several related AIGs.)</p>
+
+<p>When all of the variables in <tt>x</tt> are bound in <tt>sigma</tt>, and all
+of the values are Boolean, this is equivalent to @(see aig-eval).</p>
+
+<p>Some related functions are @(see aig-compose) and @(see
+aig-partial-eval).</p>"
+
+  (defun aig-restrict (x sigma)
+    (declare (xargs :guard t))
+    (aig-cases x
+               :true t
+               :false nil
+               :var (let ((a (hons-get x sigma)))
+                      (if a
+                          (cdr a)
+                        x))
+               :inv (aig-not (aig-restrict (car x) sigma))
+               :and (let ((a (aig-restrict (car x) sigma)))
+                      (and a (aig-and a (aig-restrict (cdr x) sigma))))))
+
+  (memoize 'aig-restrict :condition '(and (consp x) (cdr x))))
+
+
+(defsection aig-restrict-list
+  :parents (aig-restrict)
+  :short "@(call aig-restrict-list) substitutes into a list of AIGs."
+
+  (defun aig-restrict-list (x sigma)
+    (declare (xargs :guard t))
+    (if (atom x)
+        nil
+      (cons (aig-restrict (car x) sigma)
+            (aig-restrict-list (cdr x) sigma)))))
+
+
+(defsection aig-restrict-alist
+  :parents (aig-restrict)
+  :short "@(call aig-restrict-alist) substitutes into an AIG Alist (an alist
+binding keys to AIGs)."
+
+  :long "<p>The alist <tt>x</tt> does not need to be fast, and we produce an
+ordinary (slow) alist as a result.</p>"
+
+  (defun aig-restrict-alist (x sigma)
+    (declare (xargs :guard t))
+    (cond ((atom x)
+           nil)
+          ((atom (car x))
+           ;; Bad-alist convention
+           (aig-restrict-alist (cdr x) sigma))
+          (t
+           (cons (cons (caar x)
+                       (aig-restrict (cdar x) sigma))
+                 (aig-restrict-alist (cdr x) sigma)))))
+
+  (defthm alistp-of-aig-restrict-alist
+    (alistp (aig-restrict-alist x sigma))))
+
+
+(defsection aig-restrict-alists
+  :parents (aig-restrict)
+  :short "@(call aig-restrict-alists) substitutes into a list of AIG Alists."
+
+  (defun aig-restrict-alists (x sigma)
+    (declare (xargs :guard t))
+    (if (atom x)
+        nil
+      (cons (aig-restrict-alist (car x) sigma)
+            (aig-restrict-alists (cdr x) sigma)))))
+
+
+
+
+; -----------------------------------------------------------------------------
+;
+;                             AIG COMPOSITION
+;
+; -----------------------------------------------------------------------------
+
+(defsection aig-compose
+  :parents (aig)
+  :short "@(call aig-compose) performs variable substitution throughout the AIG
+<tt>x</tt>, <b>unconditionally</b> replacing every variable in <tt>x</tt> with
+its binding in <tt>sigma</tt>."
+
+  :long "<p><tt>sigma</tt> should be a fast alist; its name is intended to
+evoke the notion of substitution lists in logic.</p>
+
+<p>This function is @(see memoize)d.  You should typically free its memo table
+after you are done with whatever <tt>sigma</tt> you are using, to avoid
+excessive memory usage.  (We don't use <tt>:forget t</tt> because you often
+want to compose several related AIGs.)</p>
+
+<p>This operation is similar to @(see aig-restrict), except that whereas
+<tt>aig-restrict</tt> leaves unbound variables alone, <tt>aig-compose</tt>
+replaces them with <tt>t</tt>.  (This has the logically nice property that the
+variables after composition are just the variables in the AIGs of
+<tt>sigma</tt>.)</p>"
+
+  (defun aig-compose (x sigma)
+    (declare (xargs :guard t))
+    (aig-cases x
+               :true t
+               :false nil
+               :var (aig-env-lookup x sigma)
+               :inv (aig-not (aig-compose (car x) sigma))
+               :and (let ((a (aig-compose (car x) sigma)))
+                      (and a (aig-and a (aig-compose (cdr x) sigma))))))
+
+  (memoize 'aig-compose :condition '(and (consp x) (cdr x))))
+
+
+(defsection aig-compose-list
+  :parents (aig-compose)
+  :short "@(call aig-compose-list) composes into a list of AIGs."
+
+  (defun aig-compose-list (x sigma)
+    (declare (xargs :guard t))
+    (if (atom x)
+        nil
+      (cons (aig-compose (car x) sigma)
+            (aig-compose-list (cdr x) sigma)))))
+
+
+(defsection aig-compose-alist
+  :parents (aig-compose)
+  :short "@(call aig-compose-alist) composes into an AIG Alist (an alist
+binding keys to AIGs)."
+
+  :long "<p>The alist <tt>x</tt> does not need to be fast, and we produce an
+ordinary (slow) alist as a result.</p>"
+
+  (defun aig-compose-alist (x sigma)
+    (declare (xargs :guard t))
+    (cond ((atom x)
+           nil)
+          ((atom (car x))
+           ;; Bad alist convention
+           (aig-compose-alist (cdr x) sigma))
+          (t
+           (cons (cons (caar x)
+                       (aig-compose (cdar x) sigma))
+                 (aig-compose-alist (cdr x) sigma))))))
+
+
+(defsection aig-compose-alists
+  :parents (aig-compose)
+  :short "@(call aig-compose-alists) composes into a list of AIG Alists."
+
+  (defn aig-compose-alists (x sigma)
+    (if (atom x)
+        nil
+      (cons (aig-compose-alist (car x) sigma)
+            (aig-compose-alists (cdr x) sigma)))))
+
+
+
+; -----------------------------------------------------------------------------
+;
+;                      PARTIALLY EVALUATING AIGS
+;
+; -----------------------------------------------------------------------------
+
+(defsection aig-partial-eval
+  :parents (aig)
+  :short "@(call aig-partial-eval) evaluates <tt>x</tt>, an AIG, under the
+partial environment <tt>env</tt>, producing a new AIG as a result."
+
+  :long "<p><tt>env</tt> should be a fast alist that binds some of the
+variables in the AIG to Boolean values.</p>
+
+<p>This function is @(see memoize)d.  You should typically free its memo table
+after you are done with whatever <tt>env</tt> you are using, to avoid excessive
+memory usage.  (We don't use <tt>:forget t</tt> because you often want to
+evaluate several related AIGs.)</p>
+
+<p>In ordinary AIG evaluation with @(see aig-eval), any variables that are
+missing from <tt>env</tt> are just assumed to have a default value.  Because
+of this, every variable can be given a Boolean value and we can evaluate the
+whole AIG to produce a Boolean result.</p>
+
+<p>In partial evaluation, variables that aren't bound in <tt>env</tt> are left
+alone.  Because of this, the result of a partial evaluation is a
+new (presumably smaller) AIG, instead of a Boolean.</p>
+
+<p>Another way to do partial evaluations is with @(see aig-restrict).  The only
+difference between <tt>aig-restrict</tt> and <tt>aig-partial-eval</tt> is that
+<tt>aig-partial-eval</tt> Boolean-fixes the values in the alist as it looks
+them up.  This has logically nice properties, e.g., since we never replace a
+variable by a subtree, only by a Boolean, we know unconditionally that the
+variables of the resulting AIG are a subset of the variables of the
+original.</p>"
+
+  (defun aig-partial-eval (x env)
+    (declare (xargs :guard t))
+    (aig-cases x
+               :true t
+               :false nil
+               :var (let ((a (hons-get x env)))
+                      (if a (and (cdr a) t) x))
+               :inv (aig-not (aig-partial-eval (car x) env))
+               :and (let ((a (aig-partial-eval (car x) env)))
+                      (and a
+                           (aig-and a (aig-partial-eval (cdr x) env))))))
+
+  ;; [Jared] note: this had no memoize condition, so I added the usual one.
+
+  (memoize 'aig-partial-eval :condition '(and (consp x) (cdr x))))
+
+
+(defsection aig-partial-eval-list
+  :parents (aig-partial-eval)
+  :short "@(call aig-partial-eval-list) partially evaluates a list of AIGs."
+
+  (defun aig-partial-eval-list (x env)
+    (declare (xargs :guard t))
+    (if (atom x)
+        nil
+      (cons (aig-partial-eval (car x) env)
+            (aig-partial-eval-list (cdr x) env)))))
+
+
+(defsection aig-partial-eval-alist
+  :parents (aig-partial-eval)
+  :short "@(call aig-partial-eval-alist) partially evaluates an AIG Alist (an
+alist binding keys to AIGs)."
+
+  :long "<p>The alist <tt>x</tt> does not need to be fast, and we produce an
+ordinary (slow) alist as a result.</p>"
+
+  (defun aig-partial-eval-alist (x env)
+    (declare (xargs :guard t))
+    (cond ((atom x)
+           nil)
+          ((atom (car x))
+           ;; Bad-alist convention
+           (aig-partial-eval-alist (cdr x) env))
+          (t
+           (cons (cons (caar x)
+                       (aig-partial-eval (cdar x) env))
+                 (aig-partial-eval-alist (cdr x) env)))))
+
+  (defthm alistp-of-aig-partial-eval-alist
+    (alistp (aig-partial-eval-alist x env))))
+
+
+
+
+; -----------------------------------------------------------------------------
+;
+;                       FOUR-VALUED AIG OPERATIONS
+;
+; -----------------------------------------------------------------------------
+
+; [Jared] it would be nice to move the FAIG stuff out into a separate file.
+
+(defxdoc faig
+  :short "A representation of a four-valued function using two AIGs."
+
+  :long "<p>A <b>FAIG</b> (Four-valued AIG) combines two @(see aig)s together
+to represent a function with four possible values.  Such functions can be
+useful in hardware verification.</p>
+
+<p>We represent an FAIG as the cons of two AIGs, which are called the
+<i>onset</i> and <i>offset</i> of the FAIG.  Our FAIG evaluation function,
+@(see faig-eval), just evaluates these two AIGs, separately, using ordinary
+@(see aig-eval), and conses together the resulting Boolean values.  So, the
+four possible values of an FAIG are:</p>
+
+<ul>
+ <li><tt>(nil . nil)</tt>, which we call Z,</li>
+ <li><tt>(t . nil)</tt>, which we call True,</li>
+ <li><tt>(nil . t)</tt>, which we call False, and</li>
+ <li><tt>(t . t)</tt>, which we call X.</li>
+</ul>
+
+<p>We generally think of the onset as being a Boolean functions that should
+evaluate to <tt>T</tt> when the wire is being driven to 1.  The offset is
+similar, but indicates whether the wire is being driven to 0.  So, the Z value
+represents a situation where the wire is completely undriven, and the X value
+represents a bad case where the wire is simultaneously driven to both True and
+False.</p>
+
+<p>Hons convention.  We ordinarly construct all AIGs with @(see hons), but we
+don't bother to hons the FAIG conses that put these AIGs together.</p>
+
+<p>BOZO discuss vu-faigs too.</p>")
+
+
+; [Jared] BOZO consider a warning as in aig-eval for when faig-eval,
+; faig-restrict, etc., are used on non-consp arguments.
+
+(defsection faig-eval
+  :parents (faig)
+  :short "@(call faig-eval) evaluates <tt>x</tt>, a @(see faig), under the
+environment <tt>env</tt>, producing a pair of Boolean values."
+
+  :long "<p>See @(see aig-eval); the <tt>env</tt> should be a fast alist and
+you will want to clear the memoize table for <tt>aig-eval</tt> when you are
+done using the <tt>env</tt>.</p>"
+
+  (defun faig-eval (x env)
+    (declare (xargs :guard t))
+    (if (atom x)
+        '(t . t)
+      (cons (aig-eval (car x) env)
+            (aig-eval (cdr x) env)))))
+
+
+(defsection faig-eval-list
+  :parents (faig-eval)
+  :short "@(call faig-eval-list) evaluates a list of FAIGs."
+
+  (defun faig-eval-list (x env)
+    (declare (xargs :guard t))
+    (if (atom x)
+        nil
+      (cons (faig-eval (car x) env)
+            (faig-eval-list (cdr x) env)))))
+
+
+(defsection faig-eval-alist
+  :parents (faig-eval)
+  :short "@(call faig-eval-list) evaluates an FAIG alist (an alist binding
+keys to FAIGs)."
+
+  :long "<p>The alist <tt>x</tt> does not need to be fast, and we produce an
+ordinary (slow) alist as a result.</p>"
+
+  (defun faig-eval-alist (x env)
+    (declare (xargs :guard t))
+    (cond ((atom x)
+           nil)
+          ((atom (car x))
+           ;; Bad alist convention
+           (faig-eval-alist (cdr x) env))
+          (t
+           (cons (cons (caar x)
+                       (faig-eval (cdar x) env))
+                 (faig-eval-alist (cdr x) env))))))
+
+
+
+
+(defsection faig-restrict
+  :parents (faig)
+  :short "@(call faig-restrict) performs variable substitution throughout the
+FAIG <tt>x</tt>, replacing any variables bound in <tt>sigma</tt> with their
+corresponding values."
+
+  :long "<p>See @(see aig-restrict); the <tt>env</tt> should be a fast alist
+and you will want to clear the memoize table for <tt>aig-restrict</tt> when you
+are done using the <tt>env</tt>.</p>"
+
+  (defun faig-restrict (x sigma)
+    (declare (xargs :guard t))
+    (if (atom x)
+        '(t . t)
+      (cons (aig-restrict (car x) sigma)
+            (aig-restrict (cdr x) sigma)))))
+
+
+(defsection faig-restrict-alist
+  :parents (faig-restrict)
+  :short "@(call faig-restrict-alist) substitutes into an FAIG alist (an alist
+binding keys to FAIGs)."
+
+  :long "<p>The alist <tt>x</tt> does not need to be fast, and we produce an
+ordinary (slow) alist as a result.</p>"
+
+  (defun faig-restrict-alist (x sigma)
+    (declare (xargs :guard t))
+    (if (atom x)
+        nil
+      (let ((rest (faig-restrict-alist (cdr x) sigma)))
+        (if (atom (car x))
+            ;; Bad alist convention
+            rest
+          (cons (cons (caar x) (faig-restrict (cdar x) sigma))
+                rest))))))
+
+
+(defsection faig-restrict-alists
+  :parents (faig-restrict)
+  :short "@(call faig-restrict-alists) substitutes into a list of FAIG alists."
+
+  (defun faig-restrict-alists (x sigma)
+    (if (atom x)
+        nil
+      (cons (faig-restrict-alist (car x) sigma)
+            (faig-restrict-alists (cdr x) sigma)))))
+
+
+
+
+(defsection faig-compose
+  :parents (faig)
+  :short "@(call faig-compose) performs variable substitution throughout the
+FAIG <tt>x</tt>, <b>unconditionally</b> replacing every variable in <tt>x</tt>
+with its binding in <tt>sigma</tt>."
+
+  :long "<p>See @(see aig-compose); the <tt>sigma</tt> should be a fast alist
+and you will want to clear the memoize table for <tt>aig-compose</tt> when you
+are done using the <tt>env</tt>.</p>"
+
+  (defun faig-compose (x sigma)
+    (declare (xargs :guard t))
+    (if (atom x)
+        '(t . t)
+      (cons (aig-compose (car x) sigma)
+            (aig-compose (cdr x) sigma)))))
+
+
+(defsection faig-compose-alist
+  :parents (faig)
+  :short "@(call faig-compose-alist) composes into an FAIG Alist (an alist
+binding keys to FAIGs)."
+
+  :long "<p>The alist <tt>x</tt> does not need to be fast, and we produce an
+ordinary (slow) alist as a result.</p>"
+
+  (defun faig-compose-alist (x sigma)
+    (declare (xargs :guard t))
+    (if (atom x)
+        nil
+      (let ((rest (faig-compose-alist (cdr x) sigma)))
+        (if (atom (car x))
+            ;; Bad alist convention
+            rest
+          (cons (cons (caar x) (faig-compose (cdar x) sigma))
+                rest))))))
+
+
+
+
+(defsection faig-partial-eval
+  :parents (faig)
+  :short "@(call faig-partial-eval) evaluates <tt>x</tt>, an FAIG, under the
+partial environment <tt>env</tt>, producing a new FAIG as a result."
+
+  :long "<p>See @(see aig-partial-eval); the <tt>env</tt> should be a fast
+alist and you will want to clear the memoize table for
+<tt>aig-partial-eval</tt> when you are done using the <tt>env</tt>.</p>"
+
+  (defun faig-partial-eval (x env)
+    (declare (xargs :guard t))
+    (if (atom x)
+        '(t . t)
+      (cons (aig-partial-eval (car x) env)
+            (aig-partial-eval (cdr x) env)))))
+
+
+(defsection faig-partial-eval-alist
+  :parents (faig-partial-eval)
+  :short "@(call faig-partial-eval-alist) partially evaluates an FAIG alist (an
+alist binding keys to FAIGs)."
+
+  :long "<p>The alist <tt>x</tt> does not need to be fast, and we produce an
+ordinary (slow) alist as a result.</p>"
+
+  (defun faig-partial-eval-alist (x env)
+    (declare (xargs :guard t))
+    (if (atom x)
+        nil
+      (let ((rest (faig-partial-eval-alist (cdr x) env)))
+        (if (atom (car x))
+            ;; Bad alist convention
+            rest
+          (cons (cons (caar x) (faig-partial-eval (cdar x) env))
+                rest))))))
+
+
+(defsection faig-partial-eval-alists
+  :parents (faig-partial-eval)
+  :short "@(call faig-partial-eval-alists) partially evaluates a list of FAIG
+alists."
+
+  (defund faig-partial-eval-alists (x env)
+    (declare (xargs :guard t))
+    (if (atom x)
+        nil
+      (cons (faig-partial-eval-alist (car x) env)
+            (faig-partial-eval-alists (cdr x) env)))))
+
+
+
+
+(defsection faig-fix
+  :parents (faig)
+  :short "@(call faig-fix) is the identity for FAIGs, but coerces atoms to
+<tt>(t . t)</tt>, i.e., X."
+
+  :long "<p>This is sometimes when reasoning about FAIG operations.</p>"
+
+  (defun faig-fix (x)
+    (declare (xargs :guard t))
+    (if (consp x) x '(t . t))))
+
+
+(defsection faig-fix-list
+  :parents (faig-fix)
+  :short "@(call faig-fix-list) fixes every element of a list with @(see
+faig-fix)."
+
+  (defun faig-fix-list (x)
+    (declare (xargs :guard t))
+    (if (atom x)
+        nil
+      (cons (faig-fix (car x))
+            (faig-fix-list (cdr x))))))
+
+
+(defsection faig-fix-alist
+  :parents (faig-fix)
+  :short "@(call faig-fix-alist) fixes every value in an alist with @(see
+faig-fix)."
+
+  (defun faig-fix-alist (x)
+    (declare (xargs :guard t))
+    (cond ((atom x)
+           nil)
+          ((atom (car x))
+           ;; Bad-alist convention
+           (faig-fix-alist (cdr x)))
+          (t
+           (cons (cons (caar x) (faig-fix (cdar x)))
+                 (faig-fix-alist (cdr x)))))))
+
+
+
+
+
+
+;; [Jared] These might be more properly part of EMOD/ESIM
+
+(defun aig-eval-pat (pat x al)
   (declare (xargs :guard t))
-  (and *aig-env-lookup-warn-missing-binding*
-       (cw "~
-WARNING: Missing variable binding ~x0 in AIG-ENV-LOOKUP; assigning T~%"
-           name)))
-
-(local (in-theory (disable (break$))))
-
-(defun aig-env-lookup-missing-break (name)
-  (declare (xargs :guard t))
-  (and *aig-env-lookup-warn-missing-binding*
-       (prog2$ (cw "~
-WARNING: Missing variable binding ~x0 in AIG-ENV-LOOKUP; assigning T.
-To avoid this break, run (AIG-ENV-LOOKUP-MISSING-ACTION action), where action
-is NIL or :WARN.~%" name)
-               (break$))))
-
-(defmacro aig-env-lookup-missing-action (val)
-  (case val
-    ((nil) '(defattach aig-env-lookup-missing-output
-              aig-env-lookup-missing-quiet))
-    (:warn '(defattach aig-env-lookup-missing-output
-              aig-env-lookup-missing-complain))
-    (:break '(defattach aig-env-lookup-missing-output
-               aig-env-lookup-missing-break))
-    (t (er hard 'aig-env-lookup-missing-action
-           "Expected argument NIL, :WARN, or :BREAK.~%"))))
-
-(aig-env-lookup-missing-action :warn)
-
-
-(defun aig-env-lookup (x al)
-  (declare (Xargs :guard t))
-  (let ((look (hons-get x al)))
-    (if look
-        (cdr look)
-      (prog2$ (and *aig-env-lookup-warn-missing-binding*
-                   (aig-env-lookup-missing-output x))
-              t))))
-
-;; AIG-EVAL: Evaluates an AIG to a Boolean, given a fast alist that maps each
-;; variable to a Boolean.  (If any variable is not present in that alist, it is
-;; assumed to be NIL.)
-(defn aig-eval (x al)
-  (aig-cases
-   x
-   :true t
-   :false nil
-   :var (and (aig-env-lookup x al) t)
-   :inv (not (aig-eval (car x) al))
-   :and (and (aig-eval (car x) al)
-             (aig-eval (cdr x) al))))
-
-(memoize 'aig-eval :condition '(consp x))
-
-(defn faigp (x) (consp x))
-
-(defn faig-listp (x)
-  (if (consp x)
-      (and
-       (faigp (car x))
-       (faig-listp (cdr x)))
-    (null x))
-  )
-   
-(in-theory (disable aig-listp faig-listp))
-
-(defun faig-fix (x)
-  (declare (xargs :guard t))
-  (if (consp x) x '(t . t)))
-
-(defun faig-fix-list (x)
-  (declare (xargs :guard t))
-  (if (atom x)
-      nil
-    (cons (faig-fix (car x))
-          (faig-fix-list (cdr x)))))
-
-(defun faig-fix-alist (x)
-  (declare (xargs :guard t))
-  (if (atom x)
-      nil
-    (if (atom (car x))
-        (faig-fix-alist (cdr x))
-      (cons (cons (caar x) (faig-fix (cdar x)))
-            (faig-fix-alist (cdr x))))))
-
-
-(defun faig-eval (x env)
-  (declare (Xargs :guard t))
-  (if (atom x)
-      '(t . t)
-    (cons (aig-eval (car x) env)
-          (aig-eval (cdr x) env))))
+  (if pat
+      (if (atom pat)
+          (aig-eval x al)
+        (cons (aig-eval-pat (car pat) (ec-call (car x)) al)
+              (aig-eval-pat (cdr pat) (ec-call (cdr x)) al)))
+    nil))
 
 (defn faig-eval-pat (pat x al)
   (if pat
@@ -198,7 +1268,45 @@ is NIL or :WARN.~%" name)
               (faig-eval-pat (cdr pat) (ec-call (cdr x)) al)))
     nil))
 
+(defn faig-restrict-pat (pat fpat al)
+  (if pat
+      (if (atom pat)
+          (faig-restrict fpat al)
+        (cons (faig-restrict-pat (car pat) (ec-call (car fpat)) al)
+              (faig-restrict-pat (cdr pat) (ec-call (cdr fpat)) al)))
+    nil))
 
+(defn faig-compose-pat (pat fpat al)
+  (if pat
+      (if (atom pat)
+          (faig-compose fpat al)
+        (cons (faig-compose-pat (car pat) (ec-call (car fpat)) al)
+              (faig-compose-pat (cdr pat) (ec-call (cdr fpat)) al)))
+    nil))
+
+(defn faig-partial-eval-pat (pat fpat al)
+  (if pat
+      (if (atom pat)
+          (faig-partial-eval fpat al)
+        (cons (faig-partial-eval-pat (car pat) (ec-call (car fpat)) al)
+              (faig-partial-eval-pat (cdr pat) (ec-call (cdr fpat)) al)))
+    nil))
+
+
+
+
+
+;; [Jared] Can we get rid of this stuff?
+
+(defn faigp (x) (consp x))
+
+(defn faig-listp (x)
+  (if (consp x)
+      (and (faigp (car x))
+           (faig-listp (cdr x)))
+    (null x)))
+
+(in-theory (disable faig-listp))
 
 (defn aig-p (x)
   (aig-cases
@@ -227,592 +1335,205 @@ is NIL or :WARN.~%" name)
 
 
 
-(defn aig-eval-pat (pat x al)
-  (if pat
-      (if (atom pat)
-          (aig-eval x al)
-        (cons (aig-eval-pat (car pat) (ec-call (car x)) al)
-              (aig-eval-pat (cdr pat) (ec-call (cdr x)) al)))
-    nil))
 
-(defn faig-eval-list (x al)
-  (if (atom x)
-      nil
-    (cons (faig-eval (car x) al)
-          (faig-eval-list (cdr x) al))))
 
-(defn aig-eval-list (x al)
-  (if (atom x)
-      nil
-    (cons (aig-eval (car x) al)
-          (aig-eval-list (cdr x) al))))
 
-(defn aig-eval-alist (aig-al env)
-  (if (atom aig-al)
-      nil
-    (if (consp (car aig-al))
-        (cons (cons (caar aig-al) (aig-eval (cdar aig-al) env))
-              (aig-eval-alist (cdr aig-al) env))
-      (aig-eval-alist (cdr aig-al) env))))
 
-(defn faig-eval-alist (faig-al env)
-  (if (atom faig-al)
-      nil
-    (if (consp (car faig-al))
-        (cons (cons (caar faig-al)
-                    (faig-eval (cdar faig-al) env))
-              (faig-eval-alist (cdr faig-al) env))
-      (faig-eval-alist (cdr faig-al) env))))
 
 
+;; [Jared] Removed these things...
 
 
+;; Note that these next two functions are provably equal to T.
+;; (defn aigp (x)
+;;   (or
+;;    (atom x)
+;;    (and (consp x) (null (cdr x)))
+;;    (and (aigp (car x)) (aigp (cdr x))))
+;;   )
 
+;; (defn aig-listp (x)
+;;   (if (consp x)
+;;       (and
+;;        (aigp (car x))
+;;        (aig-listp (cdr x)))
+;;     t))
 
-;; AIG-NOT and AIG-AND are correct with respect to AIG-EVAL.
-(defthm aig-eval-not
-  (iff (aig-eval (aig-not x) al)
-       (not (aig-eval x al))))
 
-(defthm aig-eval-and
-  (iff (aig-eval (aig-and x y) al)
-       (and (aig-eval x al)
-            (aig-eval y al))))
+;; [Jared] this was never used anywhere, i think it's not necessary since
+;; aig-compose uses aig-env-lookup
 
-(in-theory (disable aig-and aig-not))
+;; (defconst *aig-compose-warn-missing-binding* t)
 
 
 
-;; Derived operators OR, ITE, XOR, IFF and correctness theorems with respec to
-;; AIG-EVAL
-(defn aig-or (x y)
-  (aig-not (aig-and (aig-not x) (aig-not y))))
 
-(defthm aig-eval-or
-  (iff (aig-eval (aig-or x y) al)
-       (or (aig-eval x al)
-           (aig-eval y al))))
 
-(in-theory (disable aig-or))
+;; [jared] this macro stuff was just used in one old mmx property checking
+;; thing it might be reasonable to put in xxxjoin style macros for aig-and,
+;; aig-or, etc.; could also implement the lazy evaluation stuff like in ubdds,
+;; if desired.
 
-(defn aig-ite (a b c)
-  (cond ((hons-equal b c)
-         b)
-        ((eq b t)
-         (aig-or a c))
-        (t (aig-or (aig-and a b)
-                   (aig-and (aig-not a) c)))))
+;; ;---- some macros for aig-or/aig-and/... 
+;; ;do we want to rebalance it (make it less deep and smaller)?
+;; ; would rebalancing have any impact on zz-sat performance?
+;; (defn aig-and-fn (lst)
+;;   (if (consp lst)
+;;       (if (consp (cdr lst))
+;;           (list
+;;            'aig-and
+;;            (car lst)
+;;            (aig-and-fn (cdr lst)))
+;;         (car lst))
+;;     t)
+;;   )
 
+;; (defmacro aig-and-macro (&rest args) (aig-and-fn args))
 
-(defthm aig-eval-ite
-  (iff (aig-eval (aig-ite a b c) al)
-       (if (aig-eval a al)
-           (aig-eval b al)
-         (aig-eval c al))))
+;; (defn aig-or-fn (lst)
+;;   (if (consp lst)
+;;       (if (consp (cdr lst))
+;;           (list
+;;            'aig-or
+;;            (car lst)
+;;            (aig-or-fn (cdr lst)))
+;;         (car lst))
+;;     nil)
+;;   )
 
+;; (defmacro aig-or-macro (&rest args) (aig-or-fn args))
 
-(defn aig-xor (a b)
-  (aig-or (aig-and a (aig-not b))
-          (aig-and (aig-not a) b)))
+;; (defn one-hot-fn (lst)
+;;   (if (consp lst)
+;;       (if (consp (cdr lst))
+;;           `(aig-or
+;;             (aig-and 
+;;              ,(car lst) 
+;;              (aig-not ,(aig-or-fn (cdr lst))))
+;;             (aig-and
+;;              (aig-not ,(car lst))
+;;              ,(one-hot-fn (cdr lst))))
+;;         (car lst))
+;;     nil
+;;     )
+;;   )
 
-(defn aig-iff (a b)
-  (aig-or (aig-and a b)
-          (aig-and (aig-not a) (aig-not b))))
+;; (defmacro one-hot (&rest args) (one-hot-fn args))
 
-(defthm aig-eval-xor
-  (iff (aig-eval (aig-xor a b) al)
-       (xor (aig-eval a al)
-            (aig-eval b al))))
+
+
+;; [Jared] looks like this was part of an experiment in transistor/propagate
+;; at one point, but it doesn't seem to be used anymore
+
+;; (defun aig-env-lookup-nil (x al)
+;;   (declare (Xargs :guard t))
+;;   (let ((look (hons-get x al)))
+;;     (if look
+;;         (cdr look)
+;;       (prog2$ (and *aig-env-lookup-warn-missing-binding*
+;;                    (aig-env-lookup-missing-output x))
+;;               nil))))
+
+;; (defn aig-compose-nil (x al)
+;;   (aig-cases
+;;    x
+;;    :true t
+;;    :false nil
+;;    :var (aig-env-lookup-nil x al)
+;;    :inv (aig-not (aig-compose-nil (car x) al))
+;;    :and (let ((a (aig-compose-nil (car x) al)))
+;;           (and a (aig-and a (aig-compose-nil (cdr x) al))))))
+
+;; (memoize 'aig-compose-nil :condition '(and (consp x) (cdr x)))
+
+;; (defn aig-compose-nil-alist (x-alst al)
+;;   (if (atom x-alst)
+;;       nil
+;;     (if (atom (car x-alst))
+;;         (aig-compose-nil-alist (cdr x-alst) al)
+;;       (cons (cons (caar x-alst)
+;;                   (aig-compose-nil (cdar x-alst) al))
+;;             (aig-compose-nil-alist (cdr x-alst) al)))))
+
+;; (defn aig-compose-nil-list (x al)
+;;   (if (atom x)
+;;       nil
+;;     (cons (aig-compose-nil (car x) al)
+;;           (aig-compose-nil-list (cdr x) al))))
+
+
+
+
+;; (defn faig-compose-nil (x comp-al)
+;;   (if (atom x)
+;;       '(t . t)
+;;     (cons (aig-compose-nil (car x) comp-al)
+;;           (aig-compose-nil (cdr x) comp-al))))
+
+;; (defn faig-compose-nil-pat (pat fpat al)
+;;   (if pat
+;;       (if (atom pat)
+;;           (faig-compose-nil fpat al)
+;;         (cons (faig-compose-nil-pat (car pat) (ec-call (car fpat)) al)
+;;               (faig-compose-nil-pat (cdr pat) (ec-call (cdr fpat)) al)))
+;;     nil))
+
+;; (defn faig-compose-nil-alist (al comp-al)
+;;   (if (atom al)
+;;       nil
+;;     (let ((rest (faig-compose-nil-alist (cdr al) comp-al)))
+;;       (if (atom (car al))
+;;           rest
+;;         (cons (cons (caar al) (faig-compose-nil (cdar al) comp-al))
+;;               rest)))))
+
+
+
+
+
+
+
+
+;; [Jared] This doesn't seem to be used for anything...
+
+;; ;; Translate Lisp-like terms into AIGs.
+;; (mutual-recursion
+;;  (defun logic-to-aig (tree)
+;;    (declare (xargs :measure (acl2-count tree)
+;;                    :guard t))
+;;    (if (atom tree)
+;;        tree
+;;      (case (car tree)
+;;        ((and or xor iff) (logic-to-aig-list (car tree) (cdr tree)))
+;;        (nand (aig-not (logic-to-aig-list 'and (cdr tree))))
+;;        (nor (aig-not (logic-to-aig-list 'or (cdr tree))))
+;;        (implies (and (eql (len tree) 3)
+;;                      (aig-or (aig-not (logic-to-aig (cadr tree)))
+;;                              (logic-to-aig (caddr tree)))))
+;;        (if (and (eql (len tree) 4)
+;;                 (aig-ite (logic-to-aig (cadr tree))
+;;                          (logic-to-aig (caddr tree))
+;;                          (logic-to-aig (cadddr tree)))))
+;;        (not (and (eql (len tree) 2)
+;;                  (aig-not (logic-to-aig (cadr tree))))))))
+;;  (defun logic-to-aig-list (op trees)
+;;    (declare (xargs :measure (acl2-count trees)
+;;                    :guard t))
+;;    (if (atom trees)
+;;        (case op
+;;          (xor nil)
+;;          (iff t)
+;;          (and t)
+;;          (or nil))
+;;      (let ((first (logic-to-aig (car trees)))
+;;            (rest (logic-to-aig-list op (cdr trees))))
+;;        (case op
+;;          (xor (aig-xor first rest))
+;;          (iff (aig-iff first rest))
+;;          (and (aig-and first rest))
+;;          (or (aig-or first rest)))))))
+
+;; (memoize 'logic-to-aig :condition '(consp tree))
 
-(defthm aig-eval-iff
-  (iff (aig-eval (aig-iff a b) al)
-       (iff (aig-eval a al)
-            (aig-eval b al))))
 
 
-(in-theory (disable aig-eval-xor aig-eval-iff aig-eval-ite))
-
-
-
-
-
-
-
-
-;; Replaces some variables of X with other values.  If all variables in x are
-;; keys in the alist and all their corresponding values are Boolean, this is
-;; equivalent to aig-eval.  Otherwise, this is a function composition.
-(defn aig-restrict (x al)
-  (aig-cases
-   x
-   :true t
-   :false nil
-   :var (let ((a (hons-get x al)))
-          (if a
-              (cdr a)
-            x))
-   :inv (aig-not (aig-restrict (car x) al))
-   :and (let ((a (aig-restrict (car x) al)))
-          (and a (aig-and a (aig-restrict (cdr x) al))))))
-
-(memoize 'aig-restrict :condition '(and (consp x) (cdr x)))
-
-(defn aig-restrict-alist (x-alst al)
-  (if (atom x-alst)
-      nil
-    (if (atom (car x-alst))
-        (aig-restrict-alist (cdr x-alst) al)
-      (cons (cons (caar x-alst)
-                  (aig-restrict (cdar x-alst) al))
-            (aig-restrict-alist (cdr x-alst) al)))))
-
-(defthm alistp-of-aig-restrict-alist
-  (alistp (aig-restrict-alist x-alst al)))
-
-
-(defn aig-restrict-list (x al)
-  (if (atom x)
-      nil
-    (cons (aig-restrict (car x) al)
-          (aig-restrict-list (cdr x) al))))
-
-
-(defn faig-restrict (x restr-al)
-  (if (atom x)
-      '(t . t)
-    (cons (aig-restrict (car x) restr-al)
-          (aig-restrict (cdr x) restr-al))))
-
-(defn faig-restrict-pat (pat fpat al)
-  (if pat
-      (if (atom pat)
-          (faig-restrict fpat al)
-        (cons (faig-restrict-pat (car pat) (ec-call (car fpat)) al)
-              (faig-restrict-pat (cdr pat) (ec-call (cdr fpat)) al)))
-    nil))
-
-
-(defn faig-restrict-alist (al comp-al)
-  (if (atom al)
-      nil
-    (let ((rest (faig-restrict-alist (cdr al) comp-al)))
-      (if (atom (car al))
-          rest
-        (cons (cons (caar al) (faig-restrict (cdar al) comp-al))
-              rest)))))
-
-(defn faig-restrict-alists (als restr-al)
-  (if (atom als)
-      nil
-    (cons (faig-restrict-alist (car als) restr-al)
-          (faig-restrict-alists (cdr als) restr-al))))
-
-
-
-;; aig-partial-eval is like aig-restrict, but treats the alist as
-;; Boolean-valued.  So one never replaces a variable by a subtree, only a
-;; boolean.
-(defun aig-partial-eval (x al)
-  (declare (xargs :guard t))
-  (aig-cases
-   x
-   :true t
-   :false nil
-   :var (let ((a (hons-get x al)))
-          (if a (and (cdr a) t) x))
-   :inv (aig-not (aig-partial-eval (car x) al))
-   :and (let ((a (aig-partial-eval (car x) al)))
-          (and a
-               (aig-and a (aig-partial-eval (cdr x) al))))))
-
-(memoize 'aig-partial-eval)
-
-(defn aig-partial-eval-alist (x-alst al)
-  (if (atom x-alst)
-      nil
-    (if (atom (car x-alst))
-        (aig-partial-eval-alist (cdr x-alst) al)
-      (cons (cons (caar x-alst)
-                  (aig-partial-eval (cdar x-alst) al))
-            (aig-partial-eval-alist (cdr x-alst) al)))))
-
-(defthm alistp-of-aig-partial-eval-alist
-  (alistp (aig-partial-eval-alist x-alst al)))
-
-
-(defn aig-partial-eval-list (x al)
-  (if (atom x)
-      nil
-    (cons (aig-partial-eval (car x) al)
-          (aig-partial-eval-list (cdr x) al))))
-
-
-(defn faig-partial-eval (x restr-al)
-  (if (atom x)
-      '(t . t)
-    (cons (aig-partial-eval (car x) restr-al)
-          (aig-partial-eval (cdr x) restr-al))))
-
-(defn faig-partial-eval-pat (pat fpat al)
-  (if pat
-      (if (atom pat)
-          (faig-partial-eval fpat al)
-        (cons (faig-partial-eval-pat (car pat) (ec-call (car fpat)) al)
-              (faig-partial-eval-pat (cdr pat) (ec-call (cdr fpat)) al)))
-    nil))
-
-
-(defn faig-partial-eval-alist (al comp-al)
-  (if (atom al)
-      nil
-    (let ((rest (faig-partial-eval-alist (cdr al) comp-al)))
-      (if (atom (car al))
-          rest
-        (cons (cons (caar al) (faig-partial-eval (cdar al) comp-al))
-              rest)))))
-
-(defn faig-partial-eval-alists (als restr-al)
-  (if (atom als)
-      nil
-    (cons (faig-partial-eval-alist (car als) restr-al)
-          (faig-partial-eval-alists (cdr als) restr-al))))
-
-
-
-
-
-
-(defconst *aig-compose-warn-missing-binding* t)
-
-(defn aig-compose (x al)
-  (aig-cases
-   x
-   :true t
-   :false nil
-   :var (aig-env-lookup x al)
-   :inv (aig-not (aig-compose (car x) al))
-   :and (let ((a (aig-compose (car x) al)))
-          (and a (aig-and a (aig-compose (cdr x) al))))))
-
-(memoize 'aig-compose :condition '(and (consp x) (cdr x)))
-
-(defn aig-compose-alist (x-alst al)
-  (if (atom x-alst)
-      nil
-    (if (atom (car x-alst))
-        (aig-compose-alist (cdr x-alst) al)
-      (cons (cons (caar x-alst)
-                  (aig-compose (cdar x-alst) al))
-            (aig-compose-alist (cdr x-alst) al)))))
-
-(defn aig-compose-list (x al)
-  (if (atom x)
-      nil
-    (cons (aig-compose (car x) al)
-          (aig-compose-list (cdr x) al))))
-
-
-(defn faig-compose (x comp-al)
-  (if (atom x)
-      '(t . t)
-    (cons (aig-compose (car x) comp-al)
-          (aig-compose (cdr x) comp-al))))
-
-(defn faig-compose-pat (pat fpat al)
-  (if pat
-      (if (atom pat)
-          (faig-compose fpat al)
-        (cons (faig-compose-pat (car pat) (ec-call (car fpat)) al)
-              (faig-compose-pat (cdr pat) (ec-call (cdr fpat)) al)))
-    nil))
-
-(defn faig-compose-alist (al comp-al)
-  (if (atom al)
-      nil
-    (let ((rest (faig-compose-alist (cdr al) comp-al)))
-      (if (atom (car al))
-          rest
-        (cons (cons (caar al) (faig-compose (cdar al) comp-al))
-              rest)))))
-
-
-
-(defun aig-env-lookup-nil (x al)
-  (declare (Xargs :guard t))
-  (let ((look (hons-get x al)))
-    (if look
-        (cdr look)
-      (prog2$ (and *aig-env-lookup-warn-missing-binding*
-                   (aig-env-lookup-missing-output x))
-              nil))))
-
-(defn aig-compose-nil (x al)
-  (aig-cases
-   x
-   :true t
-   :false nil
-   :var (aig-env-lookup-nil x al)
-   :inv (aig-not (aig-compose-nil (car x) al))
-   :and (let ((a (aig-compose-nil (car x) al)))
-          (and a (aig-and a (aig-compose-nil (cdr x) al))))))
-
-(memoize 'aig-compose-nil :condition '(and (consp x) (cdr x)))
-
-(defn aig-compose-nil-alist (x-alst al)
-  (if (atom x-alst)
-      nil
-    (if (atom (car x-alst))
-        (aig-compose-nil-alist (cdr x-alst) al)
-      (cons (cons (caar x-alst)
-                  (aig-compose-nil (cdar x-alst) al))
-            (aig-compose-nil-alist (cdr x-alst) al)))))
-
-(defn aig-compose-nil-list (x al)
-  (if (atom x)
-      nil
-    (cons (aig-compose-nil (car x) al)
-          (aig-compose-nil-list (cdr x) al))))
-
-
-(defn faig-compose-nil (x comp-al)
-  (if (atom x)
-      '(t . t)
-    (cons (aig-compose-nil (car x) comp-al)
-          (aig-compose-nil (cdr x) comp-al))))
-
-(defn faig-compose-nil-pat (pat fpat al)
-  (if pat
-      (if (atom pat)
-          (faig-compose-nil fpat al)
-        (cons (faig-compose-nil-pat (car pat) (ec-call (car fpat)) al)
-              (faig-compose-nil-pat (cdr pat) (ec-call (cdr fpat)) al)))
-    nil))
-
-(defn faig-compose-nil-alist (al comp-al)
-  (if (atom al)
-      nil
-    (let ((rest (faig-compose-nil-alist (cdr al) comp-al)))
-      (if (atom (car al))
-          rest
-        (cons (cons (caar al) (faig-compose-nil (cdar al) comp-al))
-              rest)))))
-
-
-
-
-
-
-
-
-(defabbrev fast-alphorder (x y)
-  (mbe :logic (alphorder x y)
-       :exec
-       (if (and (symbolp x)
-                (symbolp y))
-           (or (eq x y)
-               (not (symbol-< y x)))
-         (alphorder x y))))
-
-(defun hons-alphorder-merge (a b)
-  (declare (xargs :guard (and (atom-listp a)
-                              (atom-listp b))
-                  :guard-hints(("Goal" :in-theory (enable alphorder
-                                                          symbol-<)))
-                  :measure (+ (len a) (len b))))
-  (cond ((atom a) b)
-        ((atom b) a)
-        ((equal (car a) (car b))
-         (hons-alphorder-merge (cdr a) b))
-        ((fast-alphorder (car b) (car a))
-         (hons (car b) (hons-alphorder-merge a (cdr b))))
-        (t (hons (car a) (hons-alphorder-merge (cdr a) b)))))
-
-(memoize 'hons-alphorder-merge
-         :condition '(or (consp a) (consp b))
-         :inline nil)
-
-(defthm atom-listp-hons-alphorder-merge
-  (implies (and (atom-listp a)
-                (atom-listp b))
-           (atom-listp (hons-alphorder-merge a b)))
-  :hints(("Goal" :in-theory (enable hons-alphorder-merge
-                                    atom-listp))))
-
-(defthm member-equal-hons-alphorder-merge
-  (iff (member-equal k (hons-alphorder-merge a b))
-       (or (member-equal k a)
-           (member-equal k b))))
-
-
-
-;; Collects the variable list of X.
-(defun aig-vars (x)
-  (declare (xargs :guard t
-                  :verify-guards nil))
-  (aig-cases
-   x
-   :true nil
-   :false nil
-   :var  (hons x nil)
-   :inv (aig-vars (car x))
-   :and (hons-alphorder-merge (aig-vars (car x))
-                              (aig-vars (cdr x)))))
-
-(defthm atom-listp-aig-vars
-  (atom-listp (aig-vars x)))
-
-(verify-guards aig-vars)
-
-(memoize 'aig-vars :condition '(and (consp x) (cdr x)))
-
-
-
-
-
-
-
-
-;; Translate Lisp-like terms into AIGs.
-(mutual-recursion
- (defun logic-to-aig (tree)
-   (declare (xargs :measure (acl2-count tree)
-                   :guard t))
-   (if (atom tree)
-       tree
-     (case (car tree)
-       ((and or xor iff) (logic-to-aig-list (car tree) (cdr tree)))
-       (nand (aig-not (logic-to-aig-list 'and (cdr tree))))
-       (nor (aig-not (logic-to-aig-list 'or (cdr tree))))
-       (implies (and (eql (len tree) 3)
-                     (aig-or (aig-not (logic-to-aig (cadr tree)))
-                             (logic-to-aig (caddr tree)))))
-       (if (and (eql (len tree) 4)
-                (aig-ite (logic-to-aig (cadr tree))
-                         (logic-to-aig (caddr tree))
-                         (logic-to-aig (cadddr tree)))))
-       (not (and (eql (len tree) 2)
-                 (aig-not (logic-to-aig (cadr tree))))))))
- (defun logic-to-aig-list (op trees)
-   (declare (xargs :measure (acl2-count trees)
-                   :guard t))
-   (if (atom trees)
-       (case op
-         (xor nil)
-         (iff t)
-         (and t)
-         (or nil))
-     (let ((first (logic-to-aig (car trees)))
-           (rest (logic-to-aig-list op (cdr trees))))
-       (case op
-         (xor (aig-xor first rest))
-         (iff (aig-iff first rest))
-         (and (aig-and first rest))
-         (or (aig-or first rest)))))))
-
-(memoize 'logic-to-aig :condition '(consp tree))
-
-
-
-;---- some macros for aig-or/aig-and/... 
-;do we want to rebalance it (make it less deep and smaller)?
-; would rebalancing have any impact on zz-sat performance?
-(defn aig-and-fn (lst)
-  (if (consp lst)
-      (if (consp (cdr lst))
-          (list
-           'aig-and
-           (car lst)
-           (aig-and-fn (cdr lst)))
-        (car lst))
-    t)
-  )
-
-(defmacro aig-and-macro (&rest args) (aig-and-fn args))
-
-(defn aig-or-fn (lst)
-  (if (consp lst)
-      (if (consp (cdr lst))
-          (list
-           'aig-or
-           (car lst)
-           (aig-or-fn (cdr lst)))
-        (car lst))
-    nil)
-  )
-
-(defmacro aig-or-macro (&rest args) (aig-or-fn args))
-
-(defn one-hot-fn (lst)
-  (if (consp lst)
-      (if (consp (cdr lst))
-          `(aig-or
-            (aig-and 
-             ,(car lst) 
-             (aig-not ,(aig-or-fn (cdr lst))))
-            (aig-and
-             (aig-not ,(car lst))
-             ,(one-hot-fn (cdr lst))))
-        (car lst))
-    nil
-    )
-  )
-
-(defmacro one-hot (&rest args) (one-hot-fn args))
-  
-
-
-
-
-(defn aig-implies (x y)
-  ;; [Jared]: moved here from e4/recent.lisp, we probably want the usual
-  ;; theorems about this, etc.
-  (aig-not (aig-and x (aig-not y))))
-
-
-
-
-(defn aig-and-list (x)
-  (if (atom x)
-      t
-    (aig-and (car x) (aig-and-list (cdr x)))))
-
-(defn aig-or-list (x)
-  (if (atom x)
-      nil
-    (aig-or (car x) (aig-or-list (cdr x)))))
-
-(defn aig-and-lists (a b)
-  (if (or (atom a) (atom b))
-      nil
-    (cons (aig-and (car a) (car b))
-          (aig-and-lists (cdr a) (cdr b)))))
-
-(defn aig-or-lists (a b)
-  (if (or (atom a) (atom b))
-      nil
-    (cons (aig-or (car a) (car b))
-          (aig-or-lists (cdr a) (cdr b)))))
-
-(defn aig-iff-lists (a b)
-  (if (or (atom a) (atom b))
-      nil
-    (cons (aig-iff (car a) (car b))
-          (aig-iff-lists (cdr a) (cdr b)))))
-
-(defn aig-xor-lists (a b)
-  (if (or (atom a) (atom b))
-      nil
-    (cons (aig-xor (car a) (car b))
-          (aig-xor-lists (cdr a) (cdr b)))))
-
-(defn aig-implies-lists (a b)
-  (if (or (atom a) (atom b))
-      nil
-    (cons (aig-implies (car a) (car b))
-          (aig-implies-lists (cdr a) (cdr b)))))
-
-(defn aig-not-list (x)
-  (if (atom x)
-      nil
-    (cons (aig-not (car X))
-          (aig-not-list (cdr x)))))
