books/centaur/aig/eval-restrict.lisp
@@ -1,194 +1,359 @@
+; Centaur AIG Library
+; Copyright (C) 2008-2011 Centaur Technology
+;
+; Contact:
+;   Centaur Technology Formal Verification Group
+;   7600-C N. Capital of Texas Highway, Suite 300, Austin, TX 78731, USA.
+;   http://www.centtech.com/
+;
+; This program is free software; you can redistribute it and/or modify it under
+; the terms of the GNU General Public License as published by the Free Software
+; Foundation; either version 2 of the License, or (at your option) any later
+; version.  This program is distributed in the hope that it will be useful but
+; WITHOUT ANY WARRANTY; without even the implied warranty of MERCHANTABILITY or
+; FITNESS FOR A PARTICULAR PURPOSE.  See the GNU General Public License for
+; more details.  You should have received a copy of the GNU General Public
+; License along with this program; if not, write to the Free Software
+; Foundation, Inc., 51 Franklin Street, Suite 500, Boston, MA 02110-1335, USA.
+;
+; Original author: Sol Swords <sswords@centtech.com>
+;
+; July 2011, Jared added documentation, organized things into sections.
+
 
 (in-package "ACL2")
 
 (include-book "base")
 (include-book "aig-equivs")
-(include-book "faig-op-commutativity")
+(include-book "three-four")
 (include-book "aig-vars")
-(include-book "centaur/misc/universal-equiv" :dir :system)
-(include-book "centaur/misc/fast-alists" :dir :system)
-(include-book "centaur/misc/equal-sets" :dir :system)
 
-(set-inhibit-warnings "theory" "disable")
-
-
-
-;; Correctness of AIG-RESTRICT wrt AIG-EVAL:
-(defthm hons-assoc-equal-aig-eval-alist
-  (equal (hons-assoc-equal x (aig-eval-alist aig-al al))
-         (and (hons-assoc-equal x aig-al)
-              (cons x
-                    (aig-eval (cdr (hons-assoc-equal x aig-al)) al))))
-  :hints(("Goal" :in-theory (e/d (hons-assoc-equal)))))
-
-(defthm aig-eval-of-aig-restrict
-  (equal (aig-eval (aig-restrict x al1) al2)
-         (aig-eval x (append (aig-eval-alist al1 al2) al2)))
-  :hints(("Goal" :in-theory (enable aig-eval aig-restrict))))
-
+(in-theory (disable aig-env-lookup))
 (in-theory (disable aig-restrict))
-
-(defthm aig-eval-alist-of-aig-restrict-alist
-  (equal (aig-eval-alist (aig-restrict-alist x al1) al2)
-         (aig-eval-alist x (append (aig-eval-alist al1 al2) al2))))
-
-(defthm faig-eval-of-faig-restrict
-  (equal (faig-eval (faig-restrict x al1) al2)
-         (faig-eval x (append (aig-eval-alist al1 al2) al2)))
-  :hints(("Goal" :in-theory (enable faig-eval faig-restrict))))
-
-(in-theory (disable faig-restrict))
-
-
-(defthm faig-eval-pat-of-faig-restrict-pat
-  (equal (faig-eval-pat pat (faig-restrict-pat pat aigs al1) al2)
-         (faig-eval-pat pat aigs (append (aig-eval-alist al1 al2) al2))))
-
-(defthm faig-eval-alist-of-faig-restrict-alist
-  (equal (faig-eval-alist (faig-restrict-alist x al1) al2)
-         (faig-eval-alist x (append (aig-eval-alist al1 al2) al2))))
-
-
-
-
-
-(defthm aig-eval-of-aig-partial-eval
-  (equal (aig-eval (aig-partial-eval x al1) al2)
-         (aig-eval x (append al1 al2)))
-  :hints(("Goal" :in-theory (enable aig-eval aig-partial-eval))))
-
 (in-theory (disable aig-partial-eval))
-
-(defthm aig-eval-alist-of-aig-partial-eval-alist
-  (equal (aig-eval-alist (aig-partial-eval-alist x al1) al2)
-         (aig-eval-alist x (append al1 al2))))
-
-(defthm faig-eval-of-faig-partial-eval
-  (equal (faig-eval (faig-partial-eval x al1) al2)
-         (faig-eval x (append al1 al2)))
-  :hints(("Goal" :in-theory (enable faig-eval faig-partial-eval))))
-
-(in-theory (disable faig-partial-eval))
-
-(defthm faig-eval-pat-of-faig-partial-eval-pat
-  (equal (faig-eval-pat pat (faig-partial-eval-pat pat aigs al1) al2)
-         (faig-eval-pat pat aigs (append al1 al2))))
-
-(defthm faig-eval-alist-of-faig-partial-eval-alist
-  (equal (faig-eval-alist (faig-partial-eval-alist x al1) al2)
-         (faig-eval-alist x (append al1 al2))))
-
-
-
-(defthm aig-eval-of-aig-compose
-  (equal (aig-eval (aig-compose x al1) al2)
-         (aig-eval x (aig-eval-alist al1 al2))))
-
 (in-theory (disable aig-compose))
-
-(defthm aig-eval-alist-of-aig-compose-alist
-  (equal (aig-eval-alist (aig-compose-alist x al1) al2)
-         (aig-eval-alist x (aig-eval-alist al1 al2))))
-
-(defthm faig-eval-of-faig-compose
-  (equal (faig-eval (faig-compose x al1) al2)
-         (faig-eval x (aig-eval-alist al1 al2)))
-  :hints(("Goal" :in-theory (enable faig-eval faig-compose))))
-
-(in-theory (disable faig-compose))
-
-(defthm faig-eval-pat-of-faig-compose-pat
-  (equal (faig-eval-pat pat (faig-compose-pat pat aigs al1) al2)
-         (faig-eval-pat pat aigs (aig-eval-alist al1 al2))))
-
-(defthm faig-eval-alist-of-faig-compose-alist
-  (equal (faig-eval-alist (faig-compose-alist x al1) al2)
-         (faig-eval-alist x (aig-eval-alist al1 al2))))
-
-
 
 (set-default-hints '('(:do-not-induct t)))
 
-
-
-(defrefinement alist-equiv aig-env-equiv
-  :hints ((witness)))
-
-(defrefinement alist-equiv aig-alist-equiv
-  :hints ((witness)))
-
-(defrefinement alist-equiv faig-alist-equiv
-  :hints ((witness)))
 
 (defwitness alist-equiv-witnessing
   :predicate (not (alist-equiv al1 al2))
   :expr (not (let ((bg (alist-equiv-bad-guy al1 al2)))
                (equal (hons-assoc-equal bg al1)
                       (hons-assoc-equal bg al2))))
-  :hints ('(:use alist-equiv-when-agree-on-bad-guy
+  :hints('(:use alist-equiv-when-agree-on-bad-guy
                  :in-theory nil))
   :generalize (((alist-equiv-bad-guy al1 al2) . aeqkey)))
 
 
-(in-theory (disable aig-env-lookup))
-
-(defcong aig-env-equiv iff (aig-env-lookup key al) 2
-  :hints (("goal" :use ((:instance aig-env-equiv-necc
-                                   (x al) (y al-equiv))))))
-
-(defcong aig-env-equiv equal (aig-eval x env) 2
-  :hints (("goal" :induct t)))
-
-(defcong aig-env-equiv equal (aig-eval-alist x env) 2
-  :hints (("goal" :induct t)))
-
-(defcong aig-env-equiv equal (faig-eval x env) 2)
-
-(in-theory (disable faig-eval))
-
-(defcong aig-env-equiv equal (faig-eval-alist x env) 2
-  :hints (("goal" :induct t)))
-
-(defcong aig-env-equiv equal (faig-eval-pat pat x env) 3
-  :hints (("goal" :induct t)))
 
 (defexample aig-equiv-example
+    :pattern (aig-eval x env)
+    :templates (env)
+    :instance-rulename aig-equiv-instancing)
+
+(defexample aig-alist-equiv-aig-equiv-example
+    :pattern (aig-equiv (cdr (hons-assoc-equal k x))
+                        (cdr (hons-assoc-equal k y)))
+    :templates (k)
+    :instance-rulename aig-alist-equiv-instancing)
+
+(defexample aig-alist-equiv-example
+    :pattern (hons-assoc-equal k (aig-eval-alist x env))
+    :templates (k)
+    :instance-rulename aig-alist-equiv-instancing)
+
+(defexample aig-alist-equiv-not-hons-assoc-equal-ex
+    :pattern (not (hons-assoc-equal k x))
+    :templates (k)
+    :instance-rulename aig-alist-equiv-instancing)
+
+(defexample aig-alist-equiv-restrict-example
+  :pattern (hons-assoc-equal k (aig-restrict-alist x env))
+  :templates (k)
+  :instance-rulename aig-alist-equiv-instancing)
+
+(defexample aig-alist-equiv-compose-example
+  :pattern (hons-assoc-equal k (aig-compose-alist x env))
+  :templates (k)
+  :instance-rulename aig-alist-equiv-instancing)
+
+(defexample aig-alist-equiv-partial-eval-example
+  :pattern (hons-assoc-equal k (aig-partial-eval-alist x env))
+  :templates (k)
+  :instance-rulename aig-alist-equiv-instancing)
+
+
+
+(defcong aig-alist-equiv iff (hons-assoc-equal x al) 2
+  :hints((witness)))
+
+
+
+(defsection aig-eval-thms
+  :extension aig-eval
+
+  (local (in-theory (enable aig-eval)))
+
+  (defcong aig-equiv equal (aig-eval x env) 1
+    :hints((witness)))
+
+  (defcong aig-env-equiv iff (aig-env-lookup key al) 2
+    :hints(("Goal" :use ((:instance aig-env-equiv-necc
+                                     (x al) (y al-equiv))))))
+
+  (defcong aig-env-equiv equal (aig-eval x env) 2
+    :hints(("Goal" :induct t)))
+
+  (defthm aig-eval-append-when-not-intersecting-alist-keys
+    (implies (not (intersectp-equal (alist-keys env) (aig-vars x)))
+             (equal (aig-eval x (append env rest))
+                    (aig-eval x rest)))
+    :hints(("Goal"
+            :induct t
+            :in-theory (enable aig-env-lookup)))))
+
+
+
+
+(defsection aig-eval-alist-thms
+  :extension aig-eval-alist
+
+  (defthm hons-assoc-equal-aig-eval-alist
+    (equal (hons-assoc-equal key (aig-eval-alist x env))
+           (and (hons-assoc-equal key x)
+                (cons key
+                      (aig-eval (cdr (hons-assoc-equal key x)) env))))
+    :hints(("Goal" :induct t)))
+
+  (defcong aig-alist-equiv alist-equiv (aig-eval-alist x env) 1
+    :hints((witness)))
+
+  (defcong aig-env-equiv equal (aig-eval-alist x env) 2
+    :hints(("Goal" :induct t)))
+
+  (defcong aig-alist-equiv aig-alist-equiv (append a b) 1
+    :hints((witness)))
+
+  (defcong aig-alist-equiv aig-alist-equiv (append a b) 2
+    :hints((witness)))
+
+  (defthm aig-eval-alist-append
+    (equal (aig-eval-alist (append a b) env)
+           (append (aig-eval-alist a env)
+                   (aig-eval-alist b env)))
+    :hints(("Goal" :induct t)))
+
+  (defthm alist-keys-aig-eval-alist
+    (equal (alist-keys (aig-eval-alist a b))
+           (alist-keys a))
+    :hints(("Goal" :induct t))))
+
+
+
+
+(defsection aig-restrict-thms
+  :extension aig-restrict
+
+  (local (in-theory (enable aig-restrict)))
+
+  (defthm aig-eval-of-aig-restrict
+    (equal (aig-eval (aig-restrict x al1) al2)
+           (aig-eval x (append (aig-eval-alist al1 al2) al2)))
+    :hints(("Goal"
+            :induct t
+            :in-theory (enable aig-env-lookup))))
+
+  (defcong aig-equiv aig-equiv (aig-restrict x al) 1
+    :hints((witness :ruleset aig-equiv-witnessing)))
+
+  (defcong aig-alist-equiv aig-equiv (aig-restrict x al) 2
+    :hints((witness :ruleset aig-equiv-witnessing)))
+
+  (defcong alist-equiv equal (aig-restrict x env) 2
+    :hints(("Goal" :induct t))))
+
+
+
+(defsection aig-restrict-alist-thms
+  :extension aig-restrict-alist
+
+  (local (in-theory (enable aig-restrict-alist)))
+
+  (defthm lookup-in-aig-restrict-alist
+    (equal (hons-assoc-equal k (aig-restrict-alist x env))
+           (and (hons-assoc-equal k x)
+                (cons k (aig-restrict (cdr (hons-assoc-equal k x))
+                                      env))))
+    :hints(("Goal" :induct t)))
+
+  (defcong aig-alist-equiv aig-alist-equiv (aig-restrict-alist x al) 1
+    :hints((witness)))
+
+  (defcong aig-alist-equiv aig-alist-equiv (aig-restrict-alist x al) 2
+    :hints((witness :ruleset aig-alist-equiv-witnessing)))
+
+  (defthm aig-eval-alist-of-aig-restrict-alist
+    (equal (aig-eval-alist (aig-restrict-alist x al1) al2)
+           (aig-eval-alist x (append (aig-eval-alist al1 al2) al2)))
+    :hints(("Goal" :induct t)))
+
+  ;; No alist-keys thm?
+  )
+
+
+
+(defsection aig-restrict-aig-restrict
+  :extension aig-restrict
+
+  ;; This belongs in aig-restrict-thms, but needs our aig-restrict-alist
+  ;; reasoning to work.
+
+  (defthm aig-restrict-aig-restrict
+    (aig-equiv (aig-restrict (aig-restrict x al1) al2)
+               (aig-restrict x (append (aig-restrict-alist al1 al2) al2)))
+    :hints((witness))))
+
+
+(defsection aig-restrict-alist-aig-restrict-alist
+  :extension aig-restrict-alist
+
+  ;; Similarly we need aig-restrict-aig-restrict to prove this.
+
+  (defthm aig-restrict-alist-aig-restrict-alist
+    (aig-alist-equiv (aig-restrict-alist (aig-restrict-alist x al1) al2)
+                     (aig-restrict-alist x (append (aig-restrict-alist al1 al2) al2)))
+    :hints((witness))))
+
+
+
+
+(defsection aig-partial-eval-thms
+  :extension aig-partial-eval
+
+  (local (in-theory (enable aig-partial-eval)))
+
+  (defthm aig-eval-of-aig-partial-eval
+    (equal (aig-eval (aig-partial-eval x al1) al2)
+           (aig-eval x (append al1 al2)))
+    :hints(("Goal"
+             :induct t
+             :in-theory (enable aig-env-lookup))))
+
+  (defcong aig-equiv aig-equiv (aig-partial-eval x al) 1
+    :hints((witness :ruleset aig-equiv-witnessing)))
+
+  (defthm aig-partial-eval-aig-partial-eval
+    (aig-equiv (aig-partial-eval (aig-partial-eval x al1) al2)
+               (aig-partial-eval x (append al1 al2)))
+    :hints((witness)))
+
+  (defcong alist-equiv equal (aig-partial-eval x env) 2
+    :hints(("Goal" :induct t))))
+
+
+
+(defsection aig-partial-eval-alist-thms
+  :extension aig-partial-eval-alist
+
+  (local (in-theory (enable aig-partial-eval-alist)))
+
+  (defthm lookup-in-aig-partial-eval-alist
+    (equal (hons-assoc-equal k (aig-partial-eval-alist x env))
+           (and (hons-assoc-equal k x)
+                (cons k (aig-partial-eval (cdr (hons-assoc-equal k x))
+                                          env))))
+    :hints(("Goal" :induct t)))
+
+  (defcong aig-alist-equiv aig-alist-equiv (aig-partial-eval-alist x al) 1
+    :hints((witness)))
+
+  ;; BOZO maybe want some kind of env-equiv congruence too
+
+  (defthm aig-eval-alist-of-aig-partial-eval-alist
+    (equal (aig-eval-alist (aig-partial-eval-alist x al1) al2)
+           (aig-eval-alist x (append al1 al2)))
+    :hints(("Goal" :induct t)))
+
+  (defthm aig-partial-eval-alist-aig-partial-eval-alist
+    (aig-alist-equiv (aig-partial-eval-alist (aig-partial-eval-alist x al1) al2)
+                     (aig-partial-eval-alist x (append al1 al2)))
+    :hints((witness)))
+
+  ;; No alist-keys thm?
+  )
+
+
+
+(defsection aig-compose-thms
+  :extension aig-compose
+
+  (local (in-theory (enable aig-compose)))
+
+  (defthm aig-eval-of-aig-compose
+    (equal (aig-eval (aig-compose x al1) al2)
+           (aig-eval x (aig-eval-alist al1 al2)))
+    :hints(("Goal"
+            :induct t
+            :in-theory (enable aig-env-lookup))))
+
+  (defcong aig-equiv aig-equiv (aig-compose x al) 1
+    :hints((witness :ruleset aig-equiv-witnessing)))
+
+  (defcong aig-alist-equiv aig-equiv (aig-compose x al) 2
+    :hints((witness :ruleset aig-equiv-witnessing)))
+
+  (defcong alist-equiv equal (aig-compose x env) 2
+    :hints(("Goal"
+             :induct t
+             :in-theory (enable aig-env-lookup)))))
+
+
+
+
+(defsection aig-compose-alist-thms
+  :extension aig-compose-alist
+
+  (local (in-theory (enable aig-compose-alist)))
+
+  (defthm lookup-in-aig-compose-alist
+    (equal (hons-assoc-equal k (aig-compose-alist x env))
+           (and (hons-assoc-equal k x)
+                (cons k (aig-compose (cdr (hons-assoc-equal k x))
+                                     env))))
+    :hints(("Goal" :induct t)))
+
+  (defcong aig-alist-equiv aig-alist-equiv (aig-compose-alist x al) 1
+    :hints((witness)))
+
+  (defcong aig-alist-equiv aig-alist-equiv (aig-compose-alist x al) 2
+    :hints((witness :ruleset aig-alist-equiv-witnessing)))
+
+  (defthm aig-eval-alist-of-aig-compose-alist
+    (equal (aig-eval-alist (aig-compose-alist x al1) al2)
+           (aig-eval-alist x (aig-eval-alist al1 al2)))
+    :hints(("Goal" :induct t)))
+
+  ;; No alist-keys thm?
+  )
+
+
+;; BOZO should probably also disable FAIG-FIX
+(in-theory (disable faig-eval))
+(in-theory (disable faig-restrict))
+(in-theory (disable faig-partial-eval))
+(in-theory (disable faig-compose))
+
+
+(defexample faig-equiv-aig-eval-ex
   :pattern (aig-eval x env)
   :templates (env)
-  :instance-rulename aig-equiv-instancing)
+  :instance-rulename faig-equiv-instancing)
 
 (defexample faig-equiv-example
   :pattern (faig-eval x env)
   :templates (env)
   :instance-rulename faig-equiv-instancing)
-
-(defcong aig-equiv equal (aig-eval x env) 1
-  :hints ((witness)))
-
-(defexample aig-alist-equiv-example
-  :pattern (hons-assoc-equal k (aig-eval-alist x env))
-  :templates (k)
-  :instance-rulename aig-alist-equiv-instancing)
-
-(defexample aig-alist-equiv-aig-equiv-example
-  :pattern (aig-equiv (cdr (hons-assoc-equal k x))
-                      (cdr (hons-assoc-equal k y)))
-  :templates (k)
-  :instance-rulename aig-alist-equiv-instancing)
-
-(defexample aig-alist-equiv-not-hons-assoc-equal-ex
-  :pattern (not (hons-assoc-equal k x))
-  :templates (k)
-  :instance-rulename aig-alist-equiv-instancing)
-
-(defcong aig-alist-equiv alist-equiv (aig-eval-alist x env) 1
-  :hints ((witness)))
-
-(defcong aig-alist-equiv iff (hons-assoc-equal x al) 2
-  :hints ((witness)))
-
-(defcong faig-equiv equal (faig-eval x env) 1
-  :hints ((witness)))
 
 (defexample faig-alist-equiv-example
   :pattern (hons-assoc-equal k (faig-eval-alist x env))
@@ -206,415 +371,373 @@
   :templates (k)
   :instance-rulename faig-alist-equiv-instancing)
 
-(defthm lookup-in-faig-eval-alist
-  (equal (hons-assoc-equal k (faig-eval-alist x env))
-         (and (hons-assoc-equal k x)
-              (cons k (faig-eval (cdr (hons-assoc-equal k x)) env))))
-  :hints (("goal" :induct t)))
-
-(defcong faig-alist-equiv alist-equiv (faig-eval-alist x env) 1
-  :hints ((witness)))
-
-(defcong faig-alist-equiv iff (hons-assoc-equal x al) 2
-  :hints ((Witness)))
-
-(defcong aig-equiv aig-equiv (aig-restrict x al) 1
-  :hints ((witness :ruleset aig-equiv-witnessing)))
-
-(defcong aig-equiv aig-equiv (aig-partial-eval x al) 1
-  :hints ((witness :ruleset aig-equiv-witnessing)))
-
-(defcong aig-alist-equiv aig-equiv (aig-restrict x al) 2
-  :hints ((witness :ruleset aig-equiv-witnessing)))
-
-
-(defexample aig-alist-equiv-restrict-example
-  :pattern (hons-assoc-equal k (aig-restrict-alist x env))
-  :templates (k)
-  :instance-rulename aig-alist-equiv-instancing)
-
-(defthm lookup-in-aig-restrict-alist
-  (equal (hons-assoc-equal k (aig-restrict-alist x env))
-         (and (hons-assoc-equal k x)
-              (cons k (aig-restrict (cdr (hons-assoc-equal k x))
-                                    env))))
-  :hints (("goal" :induct t)))
-
-(defcong aig-alist-equiv aig-alist-equiv (aig-restrict-alist x al) 1
-  :hints ((witness)))
-
-(defexample aig-alist-equiv-partial-eval-example
-  :pattern (hons-assoc-equal k (aig-partial-eval-alist x env))
-  :templates (k)
-  :instance-rulename aig-alist-equiv-instancing)
-
-(defthm lookup-in-aig-partial-eval-alist
-  (equal (hons-assoc-equal k (aig-partial-eval-alist x env))
-         (and (hons-assoc-equal k x)
-              (cons k (aig-partial-eval (cdr (hons-assoc-equal k x))
-                                    env))))
-  :hints (("goal" :induct t)))
-
-(defcong aig-alist-equiv aig-alist-equiv (aig-partial-eval-alist x al) 1
-  :hints ((witness)))
-
-(defcong aig-alist-equiv aig-alist-equiv (aig-restrict-alist x al) 2
-  :hints ((witness :ruleset aig-alist-equiv-witnessing)))
-
-
-(defcong faig-equiv faig-equiv (faig-restrict x al) 1
-  :hints ((witness :ruleset faig-equiv-witnessing)))
-
-(defcong faig-equiv faig-equiv (faig-partial-eval x al) 1
-  :hints ((witness :ruleset faig-equiv-witnessing)))
-
-(defcong aig-alist-equiv faig-equiv (faig-restrict x al) 2
-  :hints ((witness :ruleset faig-equiv-witnessing)))
-
-
 (defexample faig-alist-equiv-restrict-example
   :pattern (hons-assoc-equal k (faig-restrict-alist x env))
   :templates (k)
   :instance-rulename faig-alist-equiv-instancing)
-
-(defthm lookup-in-faig-restrict-alist
-  (equal (hons-assoc-equal k (faig-restrict-alist x env))
-         (and (hons-assoc-equal k x)
-              (cons k (faig-restrict (cdr (hons-assoc-equal k x))
-                                     env))))
-  :hints (("goal" :induct t)))
-
-(defcong faig-alist-equiv faig-alist-equiv (faig-restrict-alist x al) 1
-  :hints ((witness)))
-
-(defexample faig-alist-equiv-partial-eval-example
-  :pattern (hons-assoc-equal k (faig-partial-eval-alist x env))
-  :templates (k)
-  :instance-rulename faig-alist-equiv-instancing)
-
-(defthm lookup-in-faig-partial-eval-alist
-  (equal (hons-assoc-equal k (faig-partial-eval-alist x env))
-         (and (hons-assoc-equal k x)
-              (cons k (faig-partial-eval (cdr (hons-assoc-equal k x))
-                                     env))))
-  :hints (("goal" :induct t)))
-
-(defcong faig-alist-equiv faig-alist-equiv (faig-partial-eval-alist x al) 1
-  :hints ((witness)))
-
-
-
-(defcong aig-alist-equiv faig-alist-equiv (faig-restrict-alist x al) 2
-  :hints ((witness :ruleset faig-alist-equiv-witnessing)))
-
-
-
-
-
-(defcong aig-equiv aig-equiv (aig-compose x al) 1
-  :hints ((witness :ruleset aig-equiv-witnessing)))
-
-(defcong aig-alist-equiv aig-equiv (aig-compose x al) 2
-  :hints ((witness :ruleset aig-equiv-witnessing)))
-
-(defexample aig-alist-equiv-compose-example
-  :pattern (hons-assoc-equal k (aig-compose-alist x env))
-  :templates (k)
-  :instance-rulename aig-alist-equiv-instancing)
-
-(defthm lookup-in-aig-compose-alist
-  (equal (hons-assoc-equal k (aig-compose-alist x env))
-         (and (hons-assoc-equal k x)
-              (cons k (aig-compose (cdr (hons-assoc-equal k x))
-                                    env))))
-  :hints (("goal" :induct t)))
-
-(defcong aig-alist-equiv aig-alist-equiv (aig-compose-alist x al) 1
-  :hints ((witness)))
-
-(defcong aig-alist-equiv aig-alist-equiv (aig-compose-alist x al) 2
-  :hints ((witness :ruleset aig-alist-equiv-witnessing)))
-
-
-(defcong faig-equiv faig-equiv (faig-compose x al) 1
-  :hints ((witness :ruleset faig-equiv-witnessing)))
-
-(defcong aig-alist-equiv faig-equiv (faig-compose x al) 2
-  :hints ((witness :ruleset faig-equiv-witnessing)))
-
 
 (defexample faig-alist-equiv-compose-example
   :pattern (hons-assoc-equal k (faig-compose-alist x env))
   :templates (k)
   :instance-rulename faig-alist-equiv-instancing)
 
-(defthm lookup-in-faig-compose-alist
-  (equal (hons-assoc-equal k (faig-compose-alist x env))
-         (and (hons-assoc-equal k x)
-              (cons k (faig-compose (cdr (hons-assoc-equal k x))
-                                     env))))
-  :hints (("goal" :induct t)))
+(defexample faig-alist-equiv-partial-eval-example
+  :pattern (hons-assoc-equal k (faig-partial-eval-alist x env))
+  :templates (k)
+  :instance-rulename faig-alist-equiv-instancing)
 
-(defcong faig-alist-equiv faig-alist-equiv (faig-compose-alist x al) 1
-  :hints ((witness)))
 
-(defcong aig-alist-equiv faig-alist-equiv (faig-compose-alist x al) 2
-  :hints ((witness :ruleset faig-alist-equiv-witnessing)))
 
 
+(defsection faig-eval-thms
+  :extension faig-eval
 
+  (defcong aig-env-equiv equal (faig-eval x env) 2
+    :hints(("Goal" :in-theory (enable faig-eval))))
 
+  (defcong faig-equiv equal (faig-eval x env) 1
+    :hints((witness)))
 
+  (defthm faig-eval-append-when-not-intersecting-alist-keys
+    (implies (not (intersectp-equal (alist-keys env) (aig-vars x)))
+             (equal (faig-eval x (append env rest))
+                    (faig-eval x rest)))
+    :hints(("Goal"
+            :in-theory (e/d (faig-eval) (aig-eval))))))
 
-(defcong aig-equiv faig-equiv (cons a b) 1
-  :hints (("goal" :in-theory (enable faig-eval))
-          (witness)))
 
-(defcong aig-equiv faig-equiv (cons a b) 2
-  :hints (("goal" :in-theory (enable faig-eval))
-          (witness)))
 
+(defsection faig-equiv-thms
+  :extension faig-equiv
 
+  (local (in-theory (enable faig-eval)))
 
-(def-universal-equiv faig-fix-equiv
-  :equiv-terms ((iff (consp x))
-                (faig-equiv x)))
+  (defcong aig-equiv faig-equiv (cons a b) 1
+    :hints((witness)))
 
-(defrefinement faig-fix-equiv faig-equiv
-  :hints(("Goal" :in-theory (enable faig-fix-equiv))))
+  (defcong aig-equiv faig-equiv (cons a b) 2
+    :hints((witness))))
 
-(defcong faig-equiv faig-fix-equiv (faig-fix x) 1
-  :hints(("Goal" :in-theory (enable faig-fix faig-fix-equiv
-                                    faig-eval))
-         (witness :ruleset (faig-equiv-witnessing
-                            faig-equiv-instancing
-                            faig-equiv-example)))
-  :otf-flg t)
 
 
-(defexample faig-equiv-aig-eval-ex
-  :pattern (aig-eval x env)
-  :templates (env)
-  :instance-rulename faig-equiv-instancing)
+(defsection faig-alist-equiv-thms
+  :extension faig-alist-equiv
 
-(defcong faig-fix-equiv aig-equiv (car x) 1
-  :hints(("Goal" :in-theory (enable faig-eval faig-fix-equiv))
-         (witness :ruleset (aig-equiv-witnessing
-                            faig-equiv-instancing
-                            faig-equiv-aig-eval-ex))))
+  (defcong faig-alist-equiv iff (hons-assoc-equal x al) 2
+    :hints((witness)))
 
-(defcong faig-fix-equiv aig-equiv (cdr x) 1
-  :hints(("Goal" :in-theory (enable faig-eval faig-fix-equiv))
-         (witness :ruleset (aig-equiv-witnessing
-                            faig-equiv-instancing
-                            faig-equiv-aig-eval-ex))))
+  (defcong faig-alist-equiv faig-alist-equiv (append a b) 1
+    :hints((witness)))
 
+  (defcong faig-alist-equiv faig-alist-equiv (append a b) 2
+    :hints((witness))))
 
-(defcong faig-alist-equiv faig-alist-equiv (append a b) 1
-  :hints ((witness)))
 
-(defcong faig-alist-equiv faig-alist-equiv (append a b) 2
-  :hints ((witness)))
 
+(defsection faig-eval-alist-thms
+  :extension faig-eval-alist
 
-(defcong aig-alist-equiv aig-alist-equiv (append a b) 1
-  :hints ((witness)))
+  (defthm faig-eval-alist-append
+    (equal (faig-eval-alist (append a b) env)
+           (append (faig-eval-alist a env)
+                   (faig-eval-alist b env)))
+    :hints(("Goal" :induct t)))
 
-(defcong aig-alist-equiv aig-alist-equiv (append a b) 2
-  :hints ((witness)))
+  (defcong aig-env-equiv equal (faig-eval-alist x env) 2
+    :hints(("Goal" :induct t)))
 
+  (defthm lookup-in-faig-eval-alist
+    (equal (hons-assoc-equal k (faig-eval-alist x env))
+           (and (hons-assoc-equal k x)
+                (cons k (faig-eval (cdr (hons-assoc-equal k x)) env))))
+    :hints(("Goal" :induct t)))
 
-(defcong alist-equiv equal (aig-restrict x env) 2
-  :hints (("goal" :induct t
-           :in-theory (enable aig-restrict))))
+  (defcong faig-alist-equiv alist-equiv (faig-eval-alist x env) 1
+    :hints((witness)))
 
-(defcong alist-equiv equal (aig-partial-eval x env) 2
-  :hints (("goal" :induct t
-           :in-theory (enable aig-partial-eval))))
+  (defthm alist-keys-faig-eval-alist
+    (equal (alist-keys (faig-eval-alist al env))
+           (alist-keys al))
+    :hints(("Goal" :induct t))))
 
-(defcong alist-equiv equal (faig-restrict x env) 2
-  :hints(("Goal" :in-theory (enable faig-restrict))))
 
-(defcong alist-equiv equal (faig-restrict-alist x env) 2
-  :hints(("goal" :in-theory (enable faig-restrict-alist)
-          :induct (len x))))
 
+(defsection faig-restrict-thms
+  :extension faig-restrict
 
-(defcong alist-equiv equal (faig-partial-eval x env) 2
-  :hints(("Goal" :in-theory (enable faig-partial-eval))))
+  (local (in-theory (enable faig-restrict)))
 
-(defcong alist-equiv equal (faig-partial-eval-alist x env) 2
-  :hints(("goal" :in-theory (enable faig-partial-eval-alist)
-          :induct (len x))))
+  (defthm faig-eval-of-faig-restrict
+    (equal (faig-eval (faig-restrict x al1) al2)
+           (faig-eval x (append (aig-eval-alist al1 al2) al2)))
+    :hints(("Goal" :in-theory (enable faig-eval))))
 
+  (defcong aig-alist-equiv faig-equiv (faig-restrict x al) 2
+    :hints((witness :ruleset faig-equiv-witnessing)))
 
+  (defcong alist-equiv equal (faig-restrict x env) 2
+    :hints(("Goal" :in-theory (enable faig-restrict))))
 
+  (local (in-theory (disable faig-restrict)))
 
-(defcong alist-equiv equal (aig-compose x env) 2
-  :hints (("goal" :induct t
-           :in-theory (enable aig-compose
-                              aig-env-lookup))))
+  (defcong faig-equiv faig-equiv (faig-restrict x al) 1
+    :hints((witness :ruleset faig-equiv-witnessing)))
 
-(defcong alist-equiv equal (faig-compose x env) 2
-  :hints(("Goal" :in-theory (enable faig-compose))))
+  (defthm faig-restrict-faig-restrict
+    (faig-equiv (faig-restrict (faig-restrict x al1) al2)
+                (faig-restrict x (append (aig-restrict-alist al1 al2) al2)))
+    :hints((witness))))
 
-(defcong alist-equiv equal (faig-compose-alist x env) 2
-  :hints(("Goal" :in-theory (enable faig-compose-alist)
-          :induct (len x))))
 
 
+(defsection faig-restrict-alist-thms
+  :extension faig-restrict-alist
 
+  (defcong alist-equiv equal (faig-restrict-alist x env) 2
+    :hints(("Goal" :induct t)))
 
+  (defthm lookup-in-faig-restrict-alist
+    (equal (hons-assoc-equal k (faig-restrict-alist x env))
+           (and (hons-assoc-equal k x)
+                (cons k (faig-restrict (cdr (hons-assoc-equal k x))
+                                       env))))
+    :hints(("Goal" :induct t)))
 
+  (defcong faig-alist-equiv faig-alist-equiv (faig-restrict-alist x al) 1
+    :hints((witness)))
 
-(defthm aig-eval-alist-append
-  (equal (aig-eval-alist (append a b) env)
-         (append (aig-eval-alist a env)
-                 (aig-eval-alist b env)))
-  :hints (("goal" :induct t)))
+  (defthm faig-eval-alist-of-faig-restrict-alist
+    (equal (faig-eval-alist (faig-restrict-alist x al1) al2)
+           (faig-eval-alist x (append (aig-eval-alist al1 al2) al2)))
+    :hints(("Goal" :induct t)))
 
-(defthm faig-eval-alist-append
-  (equal (faig-eval-alist (append a b) env)
-         (append (faig-eval-alist a env)
-                 (faig-eval-alist b env)))
-  :hints (("goal" :induct t)))
+  (defcong aig-alist-equiv faig-alist-equiv (faig-restrict-alist x al) 2
+    :hints((witness :ruleset faig-alist-equiv-witnessing)))
 
-(defthm aig-restrict-aig-restrict
-  (aig-equiv (aig-restrict (aig-restrict x al1) al2)
-             (aig-restrict x (append (aig-restrict-alist al1 al2) al2)))
-  :hints ((witness)))
+  (defthm faig-restrict-alist-faig-restrict-alist
+    (faig-alist-equiv (faig-restrict-alist (faig-restrict-alist x al1) al2)
+                      (faig-restrict-alist x (append (aig-restrict-alist al1 al2) al2)))
+    :hints((witness)))
 
-(defthm aig-restrict-alist-aig-restrict-alist
-  (aig-alist-equiv (aig-restrict-alist (aig-restrict-alist x al1) al2)
-                   (aig-restrict-alist x (append (aig-restrict-alist al1 al2) al2)))
-  :hints ((witness)))
+  (defthm alist-keys-faig-restrict-alist
+    (equal (alist-keys (faig-restrict-alist al env))
+           (alist-keys al))
+    :hints(("Goal" :induct t))))
 
-(defthm faig-restrict-faig-restrict
-  (faig-equiv (faig-restrict (faig-restrict x al1) al2)
-              (faig-restrict x (append (aig-restrict-alist al1 al2) al2)))
-  :hints ((witness)))
 
-(defthm faig-restrict-alist-faig-restrict-alist
-  (faig-alist-equiv (faig-restrict-alist (faig-restrict-alist x al1) al2)
-                    (faig-restrict-alist x (append (aig-restrict-alist al1 al2) al2)))
-  :hints ((witness)))
 
+(defsection faig-partial-eval-thms
+  :extension faig-partial-eval
 
+  (local (in-theory (enable faig-partial-eval)))
 
-(defthm aig-partial-eval-aig-partial-eval
-  (aig-equiv (aig-partial-eval (aig-partial-eval x al1) al2)
-             (aig-partial-eval x (append al1 al2)))
-  :hints ((witness)))
+  (defthm faig-eval-of-faig-partial-eval
+    (equal (faig-eval (faig-partial-eval x al1) al2)
+           (faig-eval x (append al1 al2)))
+    :hints(("Goal" :in-theory (enable faig-eval))))
 
-(defthm aig-partial-eval-alist-aig-partial-eval-alist
-  (aig-alist-equiv (aig-partial-eval-alist (aig-partial-eval-alist x al1) al2)
-                   (aig-partial-eval-alist x (append al1 al2)))
-  :hints ((witness)))
+  (defcong alist-equiv equal (faig-partial-eval x env) 2)
 
-(defthm faig-partial-eval-faig-partial-eval
-  (faig-equiv (faig-partial-eval (faig-partial-eval x al1) al2)
-              (faig-partial-eval x (append al1 al2)))
-  :hints ((witness)))
+  (local (in-theory (disable faig-partial-eval)))
 
-(defthm faig-partial-eval-alist-faig-partial-eval-alist
-  (faig-alist-equiv (faig-partial-eval-alist (faig-partial-eval-alist x al1) al2)
-                    (faig-partial-eval-alist x (append al1 al2)))
-  :hints ((witness)))
+  (defcong faig-equiv faig-equiv (faig-partial-eval x al) 1
+    :hints((witness :ruleset faig-equiv-witnessing)))
 
+  (defthm faig-partial-eval-faig-partial-eval
+    (faig-equiv (faig-partial-eval (faig-partial-eval x al1) al2)
+                (faig-partial-eval x (append al1 al2)))
+    :hints((witness))))
 
 
 
-(defthm aig-eval-append-when-not-intersecting-alist-keys
-  (implies (not (intersectp-equal (alist-keys env) (aig-vars x)))
-           (equal (aig-eval x (append env rest))
-                  (aig-eval x rest)))
-  :hints(("Goal" :in-theory (enable aig-eval aig-env-lookup)
-          :induct t)))
+(defsection faig-partial-eval-alist-thms
+  :extension faig-partial-eval-alist
 
-(defthm faig-eval-append-when-not-intersecting-alist-keys
-  (implies (not (intersectp-equal (alist-keys env) (aig-vars x)))
-           (equal (faig-eval x (append env rest))
-                  (faig-eval x rest)))
-  :hints(("Goal" :in-theory (e/d (faig-eval) (aig-eval))
-          :do-not-induct t)))
+  (defthm faig-eval-alist-of-faig-partial-eval-alist
+    (equal (faig-eval-alist (faig-partial-eval-alist x al1) al2)
+           (faig-eval-alist x (append al1 al2)))
+    :hints(("Goal" :induct t)))
 
-(defthm alist-keys-aig-eval-alist
-  (equal (alist-keys (aig-eval-alist a b))
-         (alist-keys a))
-  :hints (("goal" :induct t)))
+  (defthm lookup-in-faig-partial-eval-alist
+    (equal (hons-assoc-equal k (faig-partial-eval-alist x env))
+           (and (hons-assoc-equal k x)
+                (cons k (faig-partial-eval (cdr (hons-assoc-equal k x))
+                                           env))))
+    :hints(("Goal" :induct t)))
 
+  (defcong faig-alist-equiv faig-alist-equiv (faig-partial-eval-alist x al) 1
+    :hints((witness)))
 
-;; doing a bunch of induction here
-(set-default-hints nil)
+  (defcong alist-equiv equal (faig-partial-eval-alist x env) 2
+    :hints(("Goal" :induct t)))
 
+  (defthm faig-partial-eval-alist-faig-partial-eval-alist
+    (faig-alist-equiv (faig-partial-eval-alist (faig-partial-eval-alist x al1) al2)
+                      (faig-partial-eval-alist x (append al1 al2)))
+    :hints((witness)))
 
+  (defthm alist-keys-faig-partial-eval-alist
+    (equal (alist-keys (faig-partial-eval-alist al env))
+           (alist-keys al))
+    :hints(("Goal" :induct t))))
 
 
-(defthm faig-restrict-faig-fix
-  (equal (faig-restrict (faig-fix x) al)
-         (faig-restrict x al))
-  :hints(("Goal" :in-theory (e/d (faig-restrict aig-restrict)))))
 
-(defthm faig-restrict-alist-faig-fix-alist
-  (equal (faig-restrict-alist (faig-fix-alist a) env)
-         (faig-restrict-alist a env))
-  :hints(("Goal" :in-theory (disable faig-fix))))
 
-(defthm faig-partial-eval-faig-fix
-  (equal (faig-partial-eval (faig-fix x) al)
-         (faig-partial-eval x al))
-  :hints(("Goal" :in-theory (e/d (faig-partial-eval aig-partial-eval)))))
+(defsection faig-compose-thms
+  :extension faig-compose
 
-(defthm faig-partial-eval-alist-faig-fix-alist
-  (equal (faig-partial-eval-alist (faig-fix-alist a) env)
-         (faig-partial-eval-alist a env))
-  :hints(("Goal" :in-theory (disable faig-fix))))
+  (local (in-theory (enable faig-compose)))
 
-(defthm hons-assoc-equal-faig-fix-alist
-  (equal (hons-assoc-equal x (faig-fix-alist a))
-         (and (hons-assoc-equal x a)
-              (cons x (faig-fix (cdr (hons-assoc-equal x a)))))))
+  (defthm faig-eval-of-faig-compose
+    (equal (faig-eval (faig-compose x al1) al2)
+           (faig-eval x (aig-eval-alist al1 al2)))
+    :hints(("Goal" :in-theory (enable faig-eval))))
 
-(defthm faig-eval-faig-fix
-  (equal (faig-eval (faig-fix x) env)
-         (faig-eval x env))
-  :hints(("Goal" :in-theory (enable faig-eval faig-fix))))
+  (local (in-theory (disable faig-compose)))
 
+  (defcong faig-equiv faig-equiv (faig-compose x al) 1
+    :hints((witness :ruleset faig-equiv-witnessing)))
 
+  (defcong aig-alist-equiv faig-equiv (faig-compose x al) 2
+    :hints((witness :ruleset faig-equiv-witnessing)))
 
+  (defcong alist-equiv equal (faig-compose x env) 2
+    :hints(("Goal" :in-theory (enable faig-compose)))))
 
 
 
-(defthm alist-keys-faig-restrict-alist
-  (equal (alist-keys (faig-restrict-alist al env))
-         (alist-keys al)))
 
-(defthm alist-keys-faig-partial-eval-alist
-  (equal (alist-keys (faig-partial-eval-alist al env))
-         (alist-keys al)))
+(defsection faig-compose-alist-thms
+  :extension faig-compose-alist
 
-(defthm alist-keys-faig-eval-alist
-  (equal (alist-keys (faig-eval-alist al env))
-         (alist-keys al)))
+  (defthm faig-eval-alist-of-faig-compose-alist
+    (equal (faig-eval-alist (faig-compose-alist x al1) al2)
+           (faig-eval-alist x (aig-eval-alist al1 al2)))
+    :hints(("Goal" :induct t)))
 
+  (defthm lookup-in-faig-compose-alist
+    (equal (hons-assoc-equal k (faig-compose-alist x env))
+           (and (hons-assoc-equal k x)
+                (cons k (faig-compose (cdr (hons-assoc-equal k x))
+                                      env))))
+    :hints(("Goal" :induct t)))
 
-(defthm hons-assoc-equal-faig-eval-alist
-  (equal (hons-assoc-equal x (faig-eval-alist al env))
-         (and (hons-assoc-equal x al)
-              (cons x (faig-eval (cdr (hons-assoc-equal x al)) env)))))
+  (defcong faig-alist-equiv faig-alist-equiv (faig-compose-alist x al) 1
+    :hints((witness)))
 
+  (defcong aig-alist-equiv faig-alist-equiv (faig-compose-alist x al) 2
+    :hints((witness :ruleset faig-alist-equiv-witnessing)))
 
-(defthm faig-restrict-alist-look
-  (equal (hons-assoc-equal x (faig-restrict-alist al env))
-         (and (hons-assoc-equal x al)
-              (cons x (faig-restrict (cdr (hons-assoc-equal x al))
-                                     env)))))
+  (defcong alist-equiv equal (faig-compose-alist x env) 2
+    :hints(("Goal" :induct t))))
 
-(defthm faig-partial-eval-alist-look
-  (equal (hons-assoc-equal x (faig-partial-eval-alist al env))
-         (and (hons-assoc-equal x al)
-              (cons x (faig-partial-eval (cdr (hons-assoc-equal x al))
-                                     env)))))
+
+
+
+(defsection faig-fix-equiv
+  :parents (faig)
+  :short "We say the objects <tt>X</tt> and <tt>Y</tt> are equivalent if they
+are (1) @(see faig-equiv), and (2) both atoms or both conses."
+
+  :long "<p>This might seem kind of strange at first, but it has some nice
+congruence properties that aren't true of ordinary @(see faig-equiv).</p>
+
+<p>In particular, FAIG operations like @(see faig-eval) and @(see
+faig-restrict) generally treat any malformed FAIGs (i.e., atoms) as \"X\", that
+is, <tt>(t . t)</tt>.  This is nice because in some sense it is conservative
+with respect to our ordinary interpretation of FAIGs.</p>
+
+<p>Unfortunately, this means that <tt>faig-equiv</tt> is <b>not</b> sufficient
+to imply that the car/cdr are @(see aig-equiv).  For instance, let <tt>x</tt>
+be 5 and let <tt>y</tt> be <tt>(t . t)</tt>.  Then, <tt>x</tt> and <tt>y</tt>
+are <tt>faig-equiv</tt>, but their cars are not <tt>aig-equiv</tt> because the
+car of <tt>x</tt> is <tt>nil</tt>, constant false, whereas the car of
+<tt>y</tt> is <tt>t</tt>, constant true.</p>
+
+<p>So, @(call faig-fix-equiv) corrects for this by insisting that <tt>x</tt>
+and <tt>y</tt> are either both atoms or both conses.  This way, the car/cdr of
+<tt>faig-fix-equiv</tt> objects are always @(see aig-equiv).</p>"
+
+  (def-universal-equiv faig-fix-equiv
+    :equiv-terms ((iff (consp x))
+                  (faig-equiv x)))
+
+  (defrefinement faig-fix-equiv faig-equiv
+    :hints(("Goal" :in-theory (enable faig-fix-equiv))))
+
+  (defcong faig-equiv faig-fix-equiv (faig-fix x) 1
+    :hints(("Goal" :in-theory (enable faig-fix faig-fix-equiv
+                                      faig-eval))
+           (witness :ruleset (faig-equiv-witnessing
+                              faig-equiv-instancing
+                              faig-equiv-example)))
+    :otf-flg t)
+
+  (defcong faig-fix-equiv aig-equiv (car x) 1
+    :hints(("Goal" :in-theory (enable faig-eval faig-fix-equiv))
+           (witness :ruleset (aig-equiv-witnessing
+                              faig-equiv-instancing
+                              faig-equiv-aig-eval-ex))))
+
+  (defcong faig-fix-equiv aig-equiv (cdr x) 1
+    :hints(("Goal" :in-theory (enable faig-eval faig-fix-equiv))
+           (witness :ruleset (aig-equiv-witnessing
+                              faig-equiv-instancing
+                              faig-equiv-aig-eval-ex)))))
+
+
+
+
+(defsection faig-fix-thms
+  :extension faig-fix
+
+  (defthm faig-eval-faig-fix
+    (equal (faig-eval (faig-fix x) env)
+           (faig-eval x env))
+    :hints(("Goal" :in-theory (enable faig-eval faig-fix))))
+
+  (defthm faig-restrict-faig-fix
+    (equal (faig-restrict (faig-fix x) al)
+           (faig-restrict x al))
+    :hints(("Goal" :in-theory (e/d (faig-restrict aig-restrict)))))
+
+  (defthm faig-partial-eval-faig-fix
+    (equal (faig-partial-eval (faig-fix x) al)
+           (faig-partial-eval x al))
+    :hints(("Goal" :in-theory (e/d (faig-partial-eval aig-partial-eval)))))
+
+  ;; BOZO faig-compose?
+  )
+
+
+(defsection faig-fix-alist-thms
+  :extension faig-fix-alist
+
+  (defthm hons-assoc-equal-faig-fix-alist
+    (equal (hons-assoc-equal x (faig-fix-alist a))
+           (and (hons-assoc-equal x a)
+                (cons x (faig-fix (cdr (hons-assoc-equal x a))))))
+    :hints(("Goal" :induct t)))
+
+  (defthm faig-restrict-alist-faig-fix-alist
+    (equal (faig-restrict-alist (faig-fix-alist a) env)
+           (faig-restrict-alist a env))
+    :hints(("Goal"
+            :induct t
+            :in-theory (disable faig-fix))))
+
+  (defthm faig-partial-eval-alist-faig-fix-alist
+    (equal (faig-partial-eval-alist (faig-fix-alist a) env)
+           (faig-partial-eval-alist a env))
+    :hints(("Goal"
+            :induct t
+            :in-theory (disable faig-fix)))))
+
+
+
+
+
 
 
 (defmacro prove-faig-congruence (f args n)
@@ -623,15 +746,17 @@
                      (concatenate 'string (symbol-name arg) "-EQUIV")
                      arg))
          (args-equiv (update-nth (1- n) arg-equiv args)))
-    `(defcong faig-equiv faig-equiv (,f . ,args) ,n
-       :hints (("goal" :in-theory (disable ,f)
-                :expand ((faig-equiv (,f . ,args)
-                                     (,f . ,args-equiv)))
-              :use ((:instance faig-equiv-necc
-                               (x ,arg) (y ,arg-equiv)
-                               (env (faig-equiv-witness
+    `(defsection nil
+       :extension ,f
+       (defcong faig-equiv faig-equiv (,f . ,args) ,n
+         :hints(("Goal" :in-theory (disable ,f)
+                 :expand ((faig-equiv (,f . ,args)
+                                      (,f . ,args-equiv)))
+                 :use ((:instance faig-equiv-necc
+                                  (x ,arg) (y ,arg-equiv)
+                                  (env (faig-equiv-witness
                                      (,f . ,args)
-                                     (,f . ,args-equiv))))))))))
+                                     (,f . ,args-equiv)))))))))))
 
 (defun prove-faig-congruences-fn (n f args)
   (if (zp n)
@@ -660,3 +785,26 @@
 (prove-faig-congruences t-aig-buf (c a))
 (prove-faig-congruences f-aig-pullup (a))
 (prove-faig-congruences f-aig-bi-buf (c a b))
+
+
+
+
+;; Pat stuff, could maybe move to EMOD/ESIM books...
+
+(defthm faig-eval-pat-of-faig-restrict-pat
+  (equal (faig-eval-pat pat (faig-restrict-pat pat aigs al1) al2)
+         (faig-eval-pat pat aigs (append (aig-eval-alist al1 al2) al2)))
+  :hints(("Goal" :induct t)))
+
+(defthm faig-eval-pat-of-faig-partial-eval-pat
+  (equal (faig-eval-pat pat (faig-partial-eval-pat pat aigs al1) al2)
+         (faig-eval-pat pat aigs (append al1 al2)))
+  :hints(("Goal" :induct t)))
+
+(defthm faig-eval-pat-of-faig-compose-pat
+  (equal (faig-eval-pat pat (faig-compose-pat pat aigs al1) al2)
+         (faig-eval-pat pat aigs (aig-eval-alist al1 al2)))
+  :hints(("Goal" :induct t)))
+
+(defcong aig-env-equiv equal (faig-eval-pat pat x env) 3
+  :hints(("Goal" :induct t)))
