books/centaur/aig/three-four.lisp
@@ -1,4 +1,25 @@
-
+; Centaur AIG Library
+; Copyright (C) 2008-2011 Centaur Technology
+;
+; Contact:
+;   Centaur Technology Formal Verification Group
+;   7600-C N. Capital of Texas Highway, Suite 300, Austin, TX 78731, USA.
+;   http://www.centtech.com/
+;
+; This program is free software; you can redistribute it and/or modify it under
+; the terms of the GNU General Public License as published by the Free Software
+; Foundation; either version 2 of the License, or (at your option) any later
+; version.  This program is distributed in the hope that it will be useful but
+; WITHOUT ANY WARRANTY; without even the implied warranty of MERCHANTABILITY or
+; FITNESS FOR A PARTICULAR PURPOSE.  See the GNU General Public License for
+; more details.  You should have received a copy of the GNU General Public
+; License along with this program; if not, write to the Free Software
+; Foundation, Inc., 51 Franklin Street, Suite 500, Boston, MA 02110-1335, USA.
+;
+; Original author: Sol Swords <sswords@centtech.com>
+;
+; July 2011, Jared added some documentation and merged in the
+; faig-op-commutativity theorems.
 
 (in-package "ACL2")
 
@@ -10,6 +31,7 @@
 (defconst *4z* (hons nil nil))
 (defconst *4t* (hons t nil))
 (defconst *4f* (hons nil t))
+
 
 (def-b*-binder faig
   ":doc-section B*-BINDERS
@@ -24,62 +46,281 @@ of the given expression.~/~/~/"
            (mv (car x) (cdr x)))))
      ,rest-expr))
 
-(defn t-aig-fix (a)
-  ;; Converts floating or u values to x values.
-  (b* (((faig a1 a0) a))
-    (cons (aig-not (aig-and a0 (aig-not a1)))
-          (aig-not (aig-and a1 (aig-not a0))))))
+
+(defxdoc faig-constructors
+  :parents (faig)
+  :short "Low-level functions for constructing FAIGs."
+
+  :long "<p>In many cases, it is possible to more efficiently construct FAIGs
+when it is known that the input FAIGs cannot evaluate to Z.  This is something
+that holds of the outputs of most logic gates, e.g., a NOT gate might produce
+an X, but it will never produce a Z.</p>
+
+<p>Because of this, we have two versions of most of our FAIG constructors.  The
+<tt>t-aig-*</tt> functions make the assumption that their inputs are
+non-floating and can never evaluate to Z, and are more efficient.  The
+<tt>f-aig-*</tt> functions do not make this assumption and can operate on any
+FAIG inputs, but are not as efficient and yield larger FAIGs.</p>")
 
 
 
-(defn t-aig-not (a)
-  (b* (((faig a1 a0) a))
-    (cons a0 a1)))
+
+; Macro to prove the FAIG constructors commute over FAIG-EVAL.
+
+(defun pfoc-faig-eval-args (args)
+  (if (atom args)
+      nil
+    (cons (list 'faig-eval (car args) 'env)
+          (pfoc-faig-eval-args (cdr args)))))
+
+(defun pfoc-arg-casesplit-list (args)
+  (if (atom args)
+      nil
+    (list* `(and stable-under-simplificationp
+                 '(:cases ((aig-eval (car ,(car args)) env))))
+           `(and stable-under-simplificationp
+                 '(:cases ((aig-eval (cdr ,(car args)) env))))
+           (pfoc-arg-casesplit-list (cdr args)))))
+
+(defmacro prove-faig-op-commutes (op args)
+  `(defthm ,(intern-in-package-of-symbol
+             (concatenate 'string "FAIG-EVAL-OF-" (symbol-name op))
+             op)
+     (equal (faig-eval (,op . ,args) env)
+            (,op . ,(pfoc-faig-eval-args args)))
+     :hints ,(pfoc-arg-casesplit-list args)))
 
 
 
-(defn f-aig-not (a)
-  (b* (((faig a1 a0) a))
-    (cons (aig-not (aig-and a1 (aig-not a0)))
-          (aig-not (aig-and a0 (aig-not a1))))))
 
 
-(defn t-aig-and (a b)
-  (b* (((faig a1 a0) a)
-       ((faig b1 b0) b))
-    (cons (aig-and a1 b1)
-          (aig-or  a0 b0))))
+(defsection t-aig-fix
+  ;; BOZO should probably rename this to f-aig-unfloat
+  :parents (faig-constructors)
+  :short "Unfloat operation, converts floating (Z) values to unknown (X)
+values."
+  :long "<p>See also @(see 4v-unfloat); this is the analagous function for
+FAIGs.</p>"
 
+  (defn t-aig-fix (a)
+    (b* (((faig a1 a0) a))
+      (cons (aig-not (aig-and a0 (aig-not a1)))
+            (aig-not (aig-and a1 (aig-not a0))))))
 
-(defn f-aig-and (a b)
-  (let ((a (t-aig-fix a))
-        (b (t-aig-fix b)))
-    (t-aig-and a b)))
-
-
-
-(defn t-aig-or (a b)
-  (b* (((faig a1 a0) a)
-       ((faig b1 b0) b))
-    (cons (aig-or  a1 b1)
-          (aig-and a0 b0))))
+  (prove-faig-op-commutes t-aig-fix (a)))
 
 
 
-(defn f-aig-or (a b)
-  (let ((a (t-aig-fix a))
-        (b (t-aig-fix b)))
-    (t-aig-or a b)))
+(defsection t-aig-not
+  :parents (faig-constructors)
+  :short "@(call t-aig-not) negates the FAIG <tt>a</tt>, assuming that it
+cannot evaluate to Z."
+
+  (defn t-aig-not (a)
+    (b* (((faig a1 a0) a))
+      (cons a0 a1)))
+
+  (prove-faig-op-commutes t-aig-not (a)))
+
+
+(defsection f-aig-not
+  :parents (faig-constructors)
+  :short "@(call f-aig-not) negates the FAIG <tt>a</tt>."
+
+  (defn f-aig-not (a)
+    (b* (((faig a1 a0) a))
+      (cons (aig-not (aig-and a1 (aig-not a0)))
+            (aig-not (aig-and a0 (aig-not a1))))))
+
+  (prove-faig-op-commutes f-aig-not (a)))
 
 
 
-(defn t-aig-xor (a b)
-  (t-aig-or (t-aig-and a (t-aig-not b))
-            (t-aig-and (t-aig-not a) b)))
 
-(defn t-aig-iff (a b)
-  (t-aig-or (t-aig-and a b)
-            (t-aig-and (t-aig-not a) (t-aig-not b))))
+(defsection t-aig-and
+  :parents (faig-constructors)
+  :short "@(call t-aig-and) <i>and</i>s together the FAIGs <tt>a</tt> and
+<tt>b</tt>, assuming they cannot evaluate to Z."
+
+  (defn t-aig-and (a b)
+    (b* (((faig a1 a0) a)
+         ((faig b1 b0) b))
+      (cons (aig-and a1 b1)
+            (aig-or  a0 b0))))
+
+  (prove-faig-op-commutes t-aig-and (a b)))
+
+(defsection f-aig-and
+  :parents (faig-constructors)
+  :short "@(call f-aig-and) <i>and</i>s together the FAIGs <tt>a</tt> and
+<tt>b</tt>."
+
+  (defn f-aig-and (a b)
+    (let ((a (t-aig-fix a))
+          (b (t-aig-fix b)))
+      (t-aig-and a b)))
+
+  (prove-faig-op-commutes f-aig-and (a b)))
+
+
+
+
+(defsection t-aig-or
+  :parents (faig-constructors)
+  :short "@(call t-aig-or) <i>or</i>s together the FAIGs <tt>a</tt> and
+<tt>b</tt>, assuming they cannot evaluate to Z."
+
+  (defn t-aig-or (a b)
+    (b* (((faig a1 a0) a)
+         ((faig b1 b0) b))
+      (cons (aig-or  a1 b1)
+            (aig-and a0 b0))))
+
+  (prove-faig-op-commutes t-aig-or (a b)))
+
+(defsection f-aig-or
+  :parents (faig-constructors)
+  :short "@(call f-aig-or) <i>or</i>s together the FAIGs <tt>a</tt> and
+<tt>b</tt>."
+
+  (defn f-aig-or (a b)
+    (let ((a (t-aig-fix a))
+          (b (t-aig-fix b)))
+      (t-aig-or a b)))
+
+  (prove-faig-op-commutes f-aig-or (a b)))
+
+
+
+(defsection t-aig-xor
+  :parents (faig-constructors)
+  :short "@(call t-aig-xor) <i>xor</i>s together the FAIGs <tt>a</tt> and
+<tt>b</tt>, assuming they cannot evaluate to Z."
+
+  (defn t-aig-xor (a b)
+    (t-aig-or (t-aig-and a (t-aig-not b))
+              (t-aig-and (t-aig-not a) b)))
+
+  (prove-faig-op-commutes t-aig-xor (a b)))
+
+(defsection f-aig-xor
+  :parents (faig-constructors)
+  :short "@(call f-aig-xor) <i>xor</i>s together the FAIGs <tt>a</tt> and
+<tt>b</tt>."
+
+  (defn f-aig-xor (a b)
+    (let ((a (t-aig-fix a))
+          (b (t-aig-fix b)))
+      (t-aig-xor a b)))
+
+  (prove-faig-op-commutes f-aig-xor (a b)))
+
+
+
+(defsection t-aig-iff
+  :parents (faig-constructors)
+  :short "@(call t-aig-iff) <i>iff</i>s together the FAIGs <tt>a</tt> and
+<tt>b</tt>, assuming they cannot evaluate to Z."
+
+  (defn t-aig-iff (a b)
+    (t-aig-or (t-aig-and a b)
+              (t-aig-and (t-aig-not a) (t-aig-not b))))
+
+  (prove-faig-op-commutes t-aig-iff (a b)))
+
+
+(defsection f-aig-iff
+  :parents (faig-constructors)
+  :short "@(call f-aig-iff) <i>iff</i>s together the FAIGs <tt>a</tt> and
+<tt>b</tt>."
+
+  (defn f-aig-iff (a b)
+    (let ((a (t-aig-fix a))
+          (b (t-aig-fix b)))
+      (t-aig-iff a b)))
+
+  (prove-faig-op-commutes f-aig-iff (a b)))
+
+
+
+
+(defsection t-aig-ite
+  :parents (faig-constructors)
+  :short "@(call t-aig-ite) constructs a (less conservative) FAIG representing
+<tt>(if c a b)</tt>, assuming these input FAIGs cannot evaluate to Z."
+
+  :long "<p>This is a less-conservative version of @(see t-aig-ite*) that emits
+<tt>a</tt> in the case that <tt>c</tt> is unknown but <tt>a = b</tt>.  See
+@(see 4v-ite) for discussion related to this issue.</p>"
+
+  (defn t-aig-ite (c a b)
+    (b* (((faig a1 a0) a)
+         ((faig b1 b0) b)
+         ((faig c1 c0) c))
+      (cons (aig-or (aig-and c1 a1)
+                    (aig-and c0 b1))
+            (aig-or (aig-and c1 a0)
+                    (aig-and c0 b0)))))
+
+  (prove-faig-op-commutes t-aig-ite (c a b)))
+
+(defsection f-aig-ite
+  :parents (faig-constructors)
+  :short "@(call f-aig-ite) constructs a (less conservative) FAIG representing
+<tt>(if c a b)</tt>."
+
+  :long "<p>This is a less-conservative version of @(see f-aig-ite*) that emits
+<tt>a</tt> in the case that <tt>c</tt> is unknown but <tt>a = b</tt>.  See
+@(see 4v-ite) for discussion related to this issue.</p>"
+
+  (defn f-aig-ite (c a b)
+    (let* ((c (t-aig-fix c))
+           (a (t-aig-fix a))
+           (b (t-aig-fix b)))
+      (t-aig-ite c a b)))
+
+  (prove-faig-op-commutes f-aig-ite (c a b)))
+
+
+
+(defsection t-aig-ite*
+  :parents (faig-constructors)
+  :short "@(call t-aig-ite*) constructs a (more conservative) FAIG representing
+<tt>(if c a b)</tt>, assuming these input FAIGs cannot evaluate to Z."
+
+  :long "<p>This is a more-conservative version of @(see t-aig-ite) that emits
+<tt>X</tt> in the case that <tt>c</tt> is unknown, even when <tt>a = b</tt>.
+See @(see 4v-ite) for discussion related to this issue.</p>"
+
+  (defn t-aig-ite* (c a b)
+    (b* (((faig a1 a0) a)
+         ((faig b1 b0) b)
+         ((faig c1 c0) c)
+         (x (aig-and c1 c0)))
+      (cons (aig-or x (aig-or (aig-and c1 a1)
+                              (aig-and c0 b1)))
+            (aig-or x (aig-or (aig-and c1 a0)
+                              (aig-and c0 b0))))))
+
+  (prove-faig-op-commutes t-aig-ite* (c a b)))
+
+(defsection f-aig-ite*
+  :parents (faig-constructors)
+  :short "@(call f-aig-ite*) constructs a (more conservative) FAIG representing
+<tt>(if c a b)</tt>, assuming these input FAIGs cannot evaluate to Z."
+
+  :long "<p>This is a more-conservative version of @(see f-aig-ite) that emits
+<tt>X</tt> in the case that <tt>c</tt> is unknown, even when <tt>a = b</tt>.
+See @(see 4v-ite) for discussion related to this issue.</p>"
+
+  (defn f-aig-ite* (c a b)
+    (let* ((c (t-aig-fix c))
+           (a (t-aig-fix a))
+           (b (t-aig-fix b)))
+      (t-aig-ite* c a b)))
+
+  (prove-faig-op-commutes f-aig-ite* (c a b)))
+
 
 
 
@@ -89,57 +330,13 @@ of the given expression.~/~/~/"
     (cons (aig-or x1 y1)
           (aig-or x0 y0))))
 
+(prove-faig-op-commutes f-aig-res (a b))
+
 (defn f-aig-wire (a b)
   (f-aig-res a b))
 
 
-(defn f-aig-xor (a b)
-  (let ((a (t-aig-fix a))
-        (b (t-aig-fix b)))
-    (t-aig-xor a b)))
 
-(defn f-aig-iff (a b)
-  (let ((a (t-aig-fix a))
-        (b (t-aig-fix b)))
-    (t-aig-iff a b)))
-
-
-
-(defn t-aig-ite (c a b)
-  (b* (((faig a1 a0) a)
-       ((faig b1 b0) b)
-       ((faig c1 c0) c))
-    (cons (aig-or (aig-and c1 a1)
-                  (aig-and c0 b1))
-          (aig-or (aig-and c1 a0)
-                  (aig-and c0 b0)))))
-
-
-
-(defn f-aig-ite (c a b)  ;;  Even if C is unknown, when A=B, then A
-  (let* ((c (t-aig-fix c))
-         (a (t-aig-fix a))
-         (b (t-aig-fix b)))
-    (t-aig-ite c a b)))
-
-
-(defn t-aig-ite* (c a b)
-  (b* (((faig a1 a0) a)
-       ((faig b1 b0) b)
-       ((faig c1 c0) c)
-       (x (aig-and c1 c0)))
-    (cons (aig-or x (aig-or (aig-and c1 a1)
-                            (aig-and c0 b1)))
-          (aig-or x (aig-or (aig-and c1 a0)
-                            (aig-and c0 b0))))))
-
-
-
-(defn f-aig-ite* (c a b) ;;  Even if C is unknown, when A=B, then A
-  (let* ((c (t-aig-fix c))
-         (a (t-aig-fix a))
-         (b (t-aig-fix b)))
-    (t-aig-ite* c a b)))
 
 
 ;; Theorem: no T-AIG-FIX needed around the answer of f-aig-ite.
@@ -175,6 +372,7 @@ of the given expression.~/~/~/"
     (cons (aig-and (aig-not float) (aig-not (aig-and set off)))
           (aig-and (aig-not float) (aig-not (aig-and set on))))))
 
+(prove-faig-op-commutes t-aig-buf (c a))
 
 
 (defn f-aig-pullup (a)
@@ -183,10 +381,13 @@ of the given expression.~/~/~/"
        (a-floating (aig-not a-not-aig-floating)))
     (cons (aig-or a-floating a1) a0)))
 
+(prove-faig-op-commutes f-aig-pullup (a))
+
 
 (defn f-aig-bi-buf (cntl in bus)
   (f-aig-wire (t-aig-buf cntl in) bus))
 
+(prove-faig-op-commutes f-aig-bi-buf (c a b))
 
 (def-ruleset f-aig-defs
   '(t-aig-fix f-aig-not f-aig-and f-aig-or f-aig-xor f-aig-iff
@@ -195,6 +396,16 @@ of the given expression.~/~/~/"
 
 (def-ruleset t-aig-defs
   '(t-aig-and t-aig-iff t-aig-ite t-aig-ite* t-aig-not t-aig-or t-aig-xor))
+
+
+
+
+
+
+
+
+
+
 
 
 
