books/xdoc/package.lsp
@@ -40,6 +40,7 @@
                        *common-lisp-symbols-from-main-lisp-package*)
              ;; Things to add:
              '(b* quit exit value defxdoc defxdoc-raw macro-args
+                  xdoc-extend
                   getprop formals justification def-bodies current-acl2-world def-body
                   access theorem untranslated-theorem guard xdoc xdoc! unquote))
    ;; Things to remove:
